Loew level Merkle tree hash function parameterization, part 1

secure_api/merkle_tree/MerkleTree.New.Low.fst
@@ -13,8 +13,6 @@ open LowStar.Regional
 open LowStar.RVector
 open LowStar.Regional.Instances
 
-open MerkleTree.New.High
-
 module HS = FStar.HyperStack
 module HST = FStar.HyperStack.ST
 module MHS = FStar.Monotonic.HyperStack
@@ -32,21 +30,17 @@ module U32 = FStar.UInt32
 module U64 = FStar.UInt64
 
 module EHS = EverCrypt.Hash
-
-type const_pointer (a:Type0) = b:CB.const_buffer a{CB.length b == 1 /\ CB.qual_of b == CB.MUTABLE}
-
-#set-options "--z3rlimit 10 --max_fuel 0 --max_ifuel 0"
-
-unfold
-noextract
-let hash_alg = MerkleTree.Spec.hash_alg
-
-val hash_size: uint32_t
-let hash_size = normalize_term (UInt32.uint_to_t (MerkleTree.Spec.hash_size))
+module MTH = MerkleTree.New.High
+module MTS = MerkleTree.Spec
 
 open Lib.IntTypes
 
-type hash = buffer uint8
+#set-options "--z3rlimit 10 --initial_fuel 0 --max_fuel 0 --initial_ifuel 0 --max_ifuel 0"
+
+type const_pointer (a:Type0) = b:CB.const_buffer a{CB.length b == 1 /\ CB.qual_of b == CB.MUTABLE}
+
+type hash_size_t = n:uint32_t{n > 0ul}
+type hash (#hsz:hash_size_t) = b:buffer uint8 { B.length b = (U32.v hsz) \/ g_is_null b }
 
 // We cannot use `Low.RVector.Instances`, where we have some general
 // typeclass instances of `regional`, e.g., if `rg:regional a` then
@@ -58,34 +52,36 @@ type hash = buffer uint8
 /// Some instantiations of `regional` used in Merkle tree
 /// 1. `hash` is regional
 
-val hash_region_of: v:hash -> GTot HH.rid
-let hash_region_of v =
+val hash_region_of: #hsz:hash_size_t -> v:hash #hsz -> GTot HH.rid
+let hash_region_of #_ v =
   B.frameOf v
 
 noextract inline_for_extraction private
-val hash_dummy: hash
-let hash_dummy = B.null
+val hash_dummy (#hsz:hash_size_t): hash #hsz
+let hash_dummy #hsz = B.null
 
-val hash_r_inv: h:HS.mem -> v:hash -> GTot Type0
-let hash_r_inv h v =
+val hash_r_inv: #hsz:hash_size_t -> h:HS.mem -> v:hash #hsz -> GTot Type0
+let hash_r_inv #hsz h v =
   B.live h v /\ B.freeable v /\
-  B.len v = hash_size
+  B.len v = hsz
 
 val hash_r_inv_reg:
+  #hsz:hash_size_t ->
   h:HS.mem -> v:hash ->
   Lemma (requires hash_r_inv h v)
-        (ensures MHS.live_region h (hash_region_of v))
-let hash_r_inv_reg h v = ()
+        (ensures MHS.live_region h (hash_region_of #hsz v))
+let hash_r_inv_reg #_ h v = ()
 
 private
-val hash_repr: Type0
-let hash_repr = High.hash
+val hash_repr (#hsz:hash_size_t): Type0
+let hash_repr #hsz = MTH.hash #(U32.v hsz)
 
-val hash_r_repr: h:HS.mem -> v:hash{hash_r_inv h v} -> GTot hash_repr
-let hash_r_repr h v = B.as_seq h v
+val hash_r_repr: #hsz:hash_size_t -> h:HS.mem -> v:hash{hash_r_inv #hsz h v} -> GTot (hash_repr #hsz)
+let hash_r_repr #_ h v = B.as_seq h v
 
 val hash_r_sep:
-  v:hash -> p:loc -> h0:HS.mem -> h1:HS.mem ->
+  #hsz:hash_size_t ->
+  v:hash #hsz -> p:loc -> h0:HS.mem -> h1:HS.mem ->
   Lemma (requires
       hash_r_inv h0 v /\
       loc_disjoint
@@ -95,22 +91,23 @@ val hash_r_sep:
   (ensures
      hash_r_inv h1 v /\
      hash_r_repr h0 v == hash_r_repr h1 v)
-let hash_r_sep v p h0 h1 =
+let hash_r_sep #_ v p h0 h1 =
   assert (loc_includes (loc_all_regions_from false (hash_region_of v))
                        (loc_buffer v));
   B.modifies_buffer_elim v p h0 h1
 
-val hash_irepr: Ghost.erased hash_repr
-let hash_irepr =
-  Ghost.hide (S.create (U32.v hash_size) (u8 0))
+val hash_irepr: #hsz:hash_size_t -> Ghost.erased (hash_repr #hsz)
+let hash_irepr #hsz =
+  Ghost.hide (S.create (U32.v hsz) (u8 0))
 
-val hash_r_alloc_p: v:hash -> GTot Type0
-let hash_r_alloc_p v = True
+val hash_r_alloc_p: #hsz:hash_size_t -> v:hash #hsz -> GTot Type0
+let hash_r_alloc_p #_ v = True
 
 private
 val hash_r_alloc:
+  #hsz:hash_size_t ->
   r:HST.erid ->
-  HST.ST hash
+  HST.ST (hash #hsz)
     (requires (fun h0 -> true))
     (ensures (fun h0 v h1 ->
       Set.subset (Map.domain (MHS.get_hmap h0))
@@ -121,20 +118,22 @@ val hash_r_alloc:
       hash_region_of v = r /\
       hash_r_repr h1 v == Ghost.reveal hash_irepr /\
       B.fresh_loc (B.loc_buffer v) h0 h1))
-let hash_r_alloc r =
-  B.malloc r (u8 0) hash_size
+let hash_r_alloc #hsz r =
+  B.malloc r (u8 0) hsz
 
 val hash_r_free:
-  v:hash ->
+  #hsz:hash_size_t ->
+  v:hash #hsz ->
   HST.ST unit
     (requires fun h0 -> hash_r_inv h0 v)
     (ensures  fun h0 _ h1 ->
       modifies (loc_all_regions_from false (hash_region_of v)) h0 h1)
-let hash_r_free v =
+let hash_r_free #_ v =
   B.free v
 
 val hash_copy:
-  src:hash -> dst:hash ->
+  #hsz:hash_size_t ->
+  src:hash #hsz -> dst:hash #hsz ->
   HST.ST unit
     (requires fun h0 ->
       hash_r_inv h0 src /\ hash_r_inv h0 dst /\
@@ -143,12 +142,12 @@ val hash_copy:
       modifies (loc_all_regions_from false (hash_region_of dst)) h0 h1 /\
       hash_r_inv h1 dst /\
       hash_r_repr h1 dst == hash_r_repr h0 src)
-let hash_copy src dst =
-  B.blit src 0ul dst 0ul hash_size
+let hash_copy #hsz src dst =
+  B.blit src 0ul dst 0ul hsz
 
 noextract inline_for_extraction
-val hreg: regional hash
-let hreg =
+val hreg: #hsz:hash_size_t -> regional (hash #hsz)
+let hreg #hsz =
   Rgl hash_region_of
       B.loc_buffer
       hash_dummy
@@ -163,42 +162,43 @@ let hreg =
       hash_r_free
 
 private
-val hcpy: copyable hash hreg
-let hcpy = Cpy hash_copy
+val hcpy: #hsz:hash_size_t -> copyable (hash #hsz) hreg
+let hcpy #_ = Cpy hash_copy
 
-type hash_vec = RV.rvector hreg
+type hash_vec (#hsz:hash_size_t) = RV.rvector (hreg #hsz)
 
 /// 2. `rvector hash` is regional
 
-val hash_vec_region_of:
-  v:hash_vec -> GTot HH.rid
-let hash_vec_region_of v = V.frameOf v
+val hash_vec_region_of: #hsz:hash_size_t -> v:hash_vec #hsz -> GTot HH.rid
+let hash_vec_region_of #_ v = V.frameOf v
 
 private
-val hash_vec_dummy: hash_vec
-let hash_vec_dummy = V.alloc_empty hash
+val hash_vec_dummy: #hsz:hash_size_t -> hash_vec #hsz
+let hash_vec_dummy #_ = V.alloc_empty hash
 
-val hash_vec_r_inv:
-  h:HS.mem -> v:hash_vec -> GTot Type0
-let hash_vec_r_inv h v = RV.rv_inv h v
+val hash_vec_r_inv: #hsz:hash_size_t -> h:HS.mem -> v:hash_vec #hsz -> GTot Type0
+let hash_vec_r_inv #_ h v = RV.rv_inv h v
 
 val hash_vec_r_inv_reg:
-  h:HS.mem -> v:hash_vec ->
+  #hsz:hash_size_t -> 
+  h:HS.mem -> v:hash_vec #hsz ->
   Lemma (requires (hash_vec_r_inv h v))
   (ensures (MHS.live_region h (hash_vec_region_of v)))
-let hash_vec_r_inv_reg h v = ()
+let hash_vec_r_inv_reg #_ h v = ()
 
 private
-val hash_vec_repr: Type0
-let hash_vec_repr = High.hash_seq
+val hash_vec_repr: #hsz:hash_size_t -> Type0
+let hash_vec_repr #hsz = MTH.hashes #(U32.v hsz)
 
 val hash_vec_r_repr:
-  h:HS.mem -> v:hash_vec{hash_vec_r_inv h v} -> GTot hash_vec_repr
-let hash_vec_r_repr h v =
+  #hsz:hash_size_t -> 
+  h:HS.mem -> v:hash_vec #hsz {hash_vec_r_inv h v} -> GTot (hash_vec_repr #hsz)
+let hash_vec_r_repr #_ h v =
   RV.as_seq h v
 
 val hash_vec_r_sep:
-  v:hash_vec -> p:loc -> h0:HS.mem -> h1:HS.mem ->
+  #hsz:hash_size_t -> 
+  v:hash_vec #hsz -> p:loc -> h0:HS.mem -> h1:HS.mem ->
   Lemma (requires (hash_vec_r_inv h0 v /\
       loc_disjoint
         (loc_all_regions_from false (hash_vec_region_of v))
@@ -206,24 +206,22 @@ val hash_vec_r_sep:
       modifies p h0 h1))
   (ensures (hash_vec_r_inv h1 v /\
      hash_vec_r_repr h0 v == hash_vec_r_repr h1 v))
-let hash_vec_r_sep v p h0 h1 =
+let hash_vec_r_sep #_ v p h0 h1 =
   RV.rv_inv_preserved v p h0 h1;
   RV.as_seq_preserved v p h0 h1
 
-val hash_vec_irepr: Ghost.erased hash_vec_repr
-let hash_vec_irepr =
-  Ghost.hide S.empty
+val hash_vec_irepr: #hsz:hash_size_t -> Ghost.erased (hash_vec_repr #hsz)
+let hash_vec_irepr #_ = Ghost.hide S.empty
 
-val hash_vec_r_alloc_p: v:hash_vec -> GTot Type0
-let hash_vec_r_alloc_p v =
-  V.size_of v = 0ul
+val hash_vec_r_alloc_p: #hsz:hash_size_t -> v:hash_vec #hsz -> GTot Type0
+let hash_vec_r_alloc_p #_ v = V.size_of v = 0ul
 
-#push-options "--max_fuel 1"
-
+#push-options "--initial_fuel 1 --max_fuel 1"
 private
 val hash_vec_r_alloc:
+  #hsz:hash_size_t -> 
   r:HST.erid ->
-  HST.ST (v:hash_vec)
+  HST.ST (v:hash_vec #hsz)
     (requires (fun h0 -> true))
     (ensures (fun h0 v h1 ->
       Set.subset (Map.domain (MHS.get_hmap h0))
@@ -234,25 +232,25 @@ val hash_vec_r_alloc:
       hash_vec_region_of v = r /\
       hash_vec_r_repr h1 v == Ghost.reveal hash_vec_irepr /\
       B.fresh_loc (V.loc_vector v) h0 h1))
-let hash_vec_r_alloc r =
+let hash_vec_r_alloc #_ r =
   let nrid = HST.new_region r in
   let ia = Rgl?.dummy hreg in
   V.alloc_reserve 1ul ia r
-
 #pop-options
 
 val hash_vec_r_free:
-  v:hash_vec ->
+  #hsz:hash_size_t -> 
+  v:hash_vec #hsz ->
   HST.ST unit
     (requires (fun h0 -> hash_vec_r_inv h0 v))
     (ensures (fun h0 _ h1 ->
       modifies (loc_all_regions_from false (hash_vec_region_of v)) h0 h1))
-let hash_vec_r_free v =
+let hash_vec_r_free #_ v =
   RV.free v
 
 noextract inline_for_extraction
-val hvreg: regional hash_vec
-let hvreg =
+val hvreg: #hsz:hash_size_t -> regional (hash_vec #hsz)
+let hvreg #_ =
   Rgl hash_vec_region_of
       V.loc_vector
       hash_vec_dummy
@@ -266,47 +264,51 @@ let hvreg =
       hash_vec_r_alloc
       hash_vec_r_free
 
-type hash_vv = RV.rvector hvreg
+type hash_vv (#hsz:hash_size_t) = RV.rvector (hvreg #hsz)
 
 noextract
-val hvvreg: regional hash_vv
-let hvvreg = RVI.vector_regional hvreg
+val hvvreg: #hsz:hash_size_t -> regional (hash_vv #hsz)
+let hvvreg #_ = RVI.vector_regional hvreg
 
 private
 val hash_vec_rv_inv_r_inv:
-  h:HS.mem -> hv:hash_vec -> i:uint32_t{i < V.size_of hv} ->
+  #hsz:hash_size_t ->
+  h:HS.mem -> hv:hash_vec #hsz -> i:uint32_t{i < V.size_of hv} ->
   Lemma (requires RV.rv_inv h hv)
         (ensures  Rgl?.r_inv hreg h (V.get h hv i))
-let hash_vec_rv_inv_r_inv h hv i = ()
+let hash_vec_rv_inv_r_inv #_ h hv i = ()
 
 private
 val hash_vv_rv_inv_r_inv:
-  h:HS.mem -> hvv:hash_vv ->
+  #hsz:hash_size_t ->
+  h:HS.mem -> hvv:hash_vv #hsz ->
   i:uint32_t -> j:uint32_t ->
   Lemma (requires RV.rv_inv h hvv /\
                   i < V.size_of hvv /\
                   j < V.size_of (V.get h hvv i))
         (ensures Rgl?.r_inv hvreg h (V.get h hvv i) /\
                  Rgl?.r_inv hreg h (V.get h (V.get h hvv i) j))
-let hash_vv_rv_inv_r_inv h hvv i j = ()
+let hash_vv_rv_inv_r_inv #_ h hvv i j = ()
 
 private
 val hash_vv_rv_inv_disjoint:
-  h:HS.mem -> hvv:hash_vv ->
+  #hsz:hash_size_t ->
+  h:HS.mem -> hvv:hash_vv #hsz ->
   i:uint32_t -> j:uint32_t -> drid:HH.rid ->
   Lemma (requires (RV.rv_inv h hvv /\
                   i < V.size_of hvv /\
                   j < V.size_of (V.get h hvv i) /\
                   HH.disjoint (Rgl?.region_of hvvreg hvv) drid))
         (ensures (HH.disjoint (Rgl?.region_of hreg (V.get h (V.get h hvv i) j)) drid))
-let hash_vv_rv_inv_disjoint h hvv i j drid =
+let hash_vv_rv_inv_disjoint #_ h hvv i j drid =
   assert (HH.disjoint (Rgl?.region_of hvreg (V.get h hvv i)) drid);
   assert (RV.rv_inv h (V.get h hvv i));
   assert (HH.disjoint (Rgl?.region_of hreg (V.get h (V.get h hvv i) j)) drid)
 
 private
 val hash_vv_rv_inv_includes:
-  h:HS.mem -> hvv:hash_vv ->
+  #hsz:hash_size_t ->
+  h:HS.mem -> hvv:hash_vv #hsz ->
   i:uint32_t -> j:uint32_t ->
   Lemma (requires (RV.rv_inv h hvv /\
                   i < V.size_of hvv /\
@@ -314,28 +316,29 @@ val hash_vv_rv_inv_includes:
         (ensures (HH.includes
                    (Rgl?.region_of hvvreg hvv)
                    (Rgl?.region_of hreg (V.get h (V.get h hvv i) j))))
-let hash_vv_rv_inv_includes h hvv i j = ()
+let hash_vv_rv_inv_includes #_ h hvv i j = ()
 
 private
 val hash_vv_as_seq_get_index:
-  h:HS.mem -> hvv:hash_vv -> i:uint32_t -> j:uint32_t ->
+  #hsz:hash_size_t ->
+  h:HS.mem -> hvv:hash_vv #hsz -> i:uint32_t -> j:uint32_t ->
   Lemma (requires (RV.rv_inv h hvv /\
                   i < V.size_of hvv /\
                   j < V.size_of (V.get h hvv i)))
         (ensures (Rgl?.r_repr hreg h (V.get h (V.get h hvv i) j) ==
                  S.index (S.index (RV.as_seq h hvv) (U32.v i)) (U32.v j)))
-
-#reset-options "--z3rlimit 20"
-let hash_vv_as_seq_get_index h hvv i j = ()
+#push-options "--z3rlimit 20"
+let hash_vv_as_seq_get_index #_ h hvv i j = ()
+#pop-options
 
 /// The Merkle tree implementation begins here.
 
 /// Utility for hashes
 
-let init_hash = hash_r_alloc
-let free_hash = hash_r_free
+let init_hash (#hsz:hash_size_t) = hash_r_alloc #hsz
+let free_hash (#hsz:hash_size_t) = hash_r_free #hsz
 
-type hash_fun_t = src1:hash -> src2:hash -> dst:hash -> HST.ST unit
+type hash_fun_t (#hsz:hash_size_t) (#hash_spec:MTS.hash_fun_t #(U32.v hsz)) = src1:hash #hsz -> src2:hash #hsz -> dst:hash #hsz -> HST.ST unit
    (requires (fun h0 ->
      Rgl?.r_inv hreg h0 src1 /\
      Rgl?.r_inv hreg h0 src2 /\
@@ -346,28 +349,14 @@ type hash_fun_t = src1:hash -> src2:hash -> dst:hash -> HST.ST unit
      Rgl?.r_inv hreg h1 dst /\
      // correctness
      S.equal (Rgl?.r_repr hreg h1 dst)
-       (High.hash_2 // This is SHA256 compression, we do not verify any other hash functions.
-         (Rgl?.r_repr hreg h0 src1)
-         (Rgl?.r_repr hreg h0 src2))
-         ))
+             (hash_spec (Rgl?.r_repr hreg h0 src1) (Rgl?.r_repr hreg h0 src2))
+     ))
 
-val hash_2: src1:hash -> src2:hash -> dst:hash -> HST.ST unit
-   (requires (fun h0 ->
-     Rgl?.r_inv hreg h0 src1 /\
-     Rgl?.r_inv hreg h0 src2 /\
-     Rgl?.r_inv hreg h0 dst))
-   (ensures (fun h0 _ h1 ->
-     // memory safety
-     modifies (B.loc_region_only false (B.frameOf dst)) h0 h1 /\
-     Rgl?.r_inv hreg h1 dst /\
-     // correctness
-     S.equal (Rgl?.r_repr hreg h1 dst)
-       (High.hash_2 // This is SHA256 compression, we do not verify any other hash functions.
-         (Rgl?.r_repr hreg h0 src1)
-         (Rgl?.r_repr hreg h0 src2))
-         ))
-#reset-options "--z3rlimit 40 --max_fuel 0"
-let hash_2 src1 src2 dst =
+val sha256_compress: hash_fun_t #32ul #MTH.sha256_compress
+#push-options "--z3rlimit 40 --max_fuel 0"
+let sha256_compress src1 src2 dst =
+  let hash_size = 32ul in
+  let hash_alg = Spec.Hash.Definitions.SHA2_256 in
   let hh0 = HST.get () in
   HST.push_frame ();
   // KreMLin can't extract `EHS.blockLen EHS.SHA256` (= 64ul)
@@ -397,21 +386,20 @@ let hash_2 src1 src2 dst =
   assert (S.equal (B.as_seq hh3 dst)
                   (Spec.Hash.PadFinish.finish hash_alg (Spec.Agile.Hash.update hash_alg (Spec.Agile.Hash.init hash_alg) (B.as_seq hh1 cb))));
   assert (S.equal (B.as_seq hh3 dst)
-                  (High.hash_2
+                  (MTH.sha256_compress
                     (Rgl?.r_repr hreg hh0 src1)
                     (Rgl?.r_repr hreg hh0 src2)));
   HST.pop_frame ();
 
   let hh4 = HST.get () in
   assert (S.equal (B.as_seq hh4 dst)
-                  (High.hash_2
+                  (MTH.sha256_compress
                     (Rgl?.r_repr hreg hh0 src1)
                     (Rgl?.r_repr hreg hh0 src2)))
+#pop-options
 
 /// Low-level Merkle tree data structure
-
-#reset-options "--z3rlimit 20"
-
+/// 
 // NOTE: because of a lack of 64-bit LowStar.Buffer support, currently
 // we cannot change below to some other types.
 type index_t = uint32_t
@@ -457,20 +445,22 @@ let merkle_tree_size_lg = 32ul
 //          root of the tree. If `rhs_ok` is true then it has the up-to-date
 //          root value.
 noeq type merkle_tree =
-| MT: offset:offset_t ->
+| MT: hash_size:hash_size_t ->
+      offset:offset_t ->
       i:index_t -> j:index_t{i <= j /\ add64_fits offset j} ->
-      hs:hash_vv{V.size_of hs = merkle_tree_size_lg} ->
+      hs:hash_vv #hash_size {V.size_of hs = merkle_tree_size_lg} ->
       rhs_ok:bool ->
-      rhs:hash_vec{V.size_of rhs = merkle_tree_size_lg} ->
-      mroot:hash ->
-      hash_fun:hash_fun_t ->
+      rhs:hash_vec #hash_size {V.size_of rhs = merkle_tree_size_lg} ->
+      mroot:hash #hash_size ->
+      hash_spec:Ghost.erased (MTS.hash_fun_t #(U32.v hash_size)) ->
+      hash_fun:hash_fun_t #hash_size #hash_spec ->
       merkle_tree
 
 type mt_p = B.pointer merkle_tree
 type const_mt_p = const_pointer merkle_tree
 
 inline_for_extraction
-let merkle_tree_conditions (offset:uint64_t) (i j:uint32_t) (hs:hash_vv) (rhs_ok:bool) (rhs:hash_vec) (mroot:hash): Tot bool =
+let merkle_tree_conditions (#hsz:hash_size_t) (offset:uint64_t) (i j:uint32_t) (hs:hash_vv #hsz) (rhs_ok:bool) (rhs:hash_vec #hsz) (mroot:hash #hsz): Tot bool =
   j >= i && add64_fits offset j &&
   V.size_of hs = merkle_tree_size_lg &&
   V.size_of rhs = merkle_tree_size_lg
@@ -480,8 +470,7 @@ let merkle_tree_conditions (offset:uint64_t) (i j:uint32_t) (hs:hash_vv) (rhs_ok
 // vector is full; this can be fixed if necessary.
 private inline_for_extraction
 val mt_not_full_nst: mtv:merkle_tree -> Tot bool
-let mt_not_full_nst mtv =
-  MT?.j mtv < uint32_32_max
+let mt_not_full_nst mtv = MT?.j mtv < uint32_32_max
 
 val mt_not_full: HS.mem -> mt_p -> GTot bool
 let mt_not_full h mt = mt_not_full_nst (B.get h mt 0)
@@ -489,78 +478,87 @@ let mt_not_full h mt = mt_not_full_nst (B.get h mt 0)
 /// (Memory) Safety
 
 val offset_of: i:index_t -> Tot index_t
-let offset_of i =
-  if i % 2ul = 0ul then i else i - 1ul
+let offset_of i = if i % 2ul = 0ul then i else i - 1ul
 
 // `mt_safe_elts` says that it is safe to access an element from `i` to `j - 1`
 // at level `lv` in the Merkle tree, i.e., hs[lv][k] (i <= k < j) is a valid
 // element.
 val mt_safe_elts:
+  #hsz:hash_size_t ->
   h:HS.mem -> lv:uint32_t{lv <= merkle_tree_size_lg} ->
-  hs:hash_vv{V.size_of hs = merkle_tree_size_lg} ->
+  hs:hash_vv #hsz {V.size_of hs = merkle_tree_size_lg} ->
   i:index_t -> j:index_t{j >= i} ->
   GTot Type0 (decreases (32 - U32.v lv))
-let rec mt_safe_elts h lv hs i j =
+let rec mt_safe_elts #hsz h lv hs i j =
   if lv = merkle_tree_size_lg then true
   else (let ofs = offset_of i in
        V.size_of (V.get h hs lv) == j - ofs /\
-       mt_safe_elts h (lv + 1ul) hs (i / 2ul) (j / 2ul))
+       mt_safe_elts #hsz h (lv + 1ul) hs (i / 2ul) (j / 2ul))
 
+#push-options "--initial_fuel 1 --max_fuel 1"
 val mt_safe_elts_constr:
+  #hsz:hash_size_t ->
   h:HS.mem -> lv:uint32_t{lv < merkle_tree_size_lg} ->
-  hs:hash_vv{V.size_of hs = merkle_tree_size_lg} ->
+  hs:hash_vv #hsz {V.size_of hs = merkle_tree_size_lg} ->
   i:index_t -> j:index_t{j >= i} ->
   Lemma (requires (V.size_of (V.get h hs lv) == j - offset_of i /\
-                  mt_safe_elts h (lv + 1ul) hs (i / 2ul) (j / 2ul)))
-        (ensures (mt_safe_elts h lv hs i j))
-let mt_safe_elts_constr h lv hs i j = ()
+                  mt_safe_elts #hsz h (lv + 1ul) hs (i / 2ul) (j / 2ul)))
+        (ensures (mt_safe_elts #hsz h lv hs i j))
+let mt_safe_elts_constr #_ h lv hs i j = ()
 
 val mt_safe_elts_head:
+  #hsz:hash_size_t ->
   h:HS.mem -> lv:uint32_t{lv < merkle_tree_size_lg} ->
-  hs:hash_vv{V.size_of hs = merkle_tree_size_lg} ->
+  hs:hash_vv #hsz {V.size_of hs = merkle_tree_size_lg} ->
   i:index_t -> j:index_t{j >= i} ->
-  Lemma (requires (mt_safe_elts h lv hs i j))
+  Lemma (requires (mt_safe_elts #hsz h lv hs i j))
         (ensures (V.size_of (V.get h hs lv) == j - offset_of i))
-let mt_safe_elts_head h lv hs i j = ()
+let mt_safe_elts_head #_ h lv hs i j = ()
 
 val mt_safe_elts_rec:
+  #hsz:hash_size_t ->
   h:HS.mem -> lv:uint32_t{lv < merkle_tree_size_lg} ->
-  hs:hash_vv{V.size_of hs = merkle_tree_size_lg} ->
+  hs:hash_vv #hsz {V.size_of hs = merkle_tree_size_lg} ->
   i:index_t -> j:index_t{j >= i} ->
-  Lemma (requires (mt_safe_elts h lv hs i j))
-        (ensures (mt_safe_elts h (lv + 1ul) hs (i / 2ul) (j / 2ul)))
-let mt_safe_elts_rec h lv hs i j = ()
+  Lemma (requires (mt_safe_elts #hsz h lv hs i j))
+        (ensures (mt_safe_elts #hsz h (lv + 1ul) hs (i / 2ul) (j / 2ul)))
+let mt_safe_elts_rec #_ h lv hs i j = ()
 
 val mt_safe_elts_init:
+  #hsz:hash_size_t ->
   h:HS.mem -> lv:uint32_t{lv <= merkle_tree_size_lg} ->
-  hs:hash_vv{V.size_of hs = merkle_tree_size_lg} ->
+  hs:hash_vv #hsz {V.size_of hs = merkle_tree_size_lg} ->
   Lemma (requires (V.forall_ h hs lv (V.size_of hs)
                     (fun hv -> V.size_of hv = 0ul)))
-        (ensures (mt_safe_elts h lv hs 0ul 0ul))
+        (ensures (mt_safe_elts #hsz h lv hs 0ul 0ul))
         (decreases (32 - U32.v lv))
-let rec mt_safe_elts_init h lv hs =
+let rec mt_safe_elts_init #hsz h lv hs =
   if lv = merkle_tree_size_lg then ()
-  else mt_safe_elts_init h (lv + 1ul) hs
+  else mt_safe_elts_init #hsz h (lv + 1ul) hs
+#pop-options
 
 val mt_safe_elts_preserved:
+  #hsz:hash_size_t ->
   lv:uint32_t{lv <= merkle_tree_size_lg} ->
-  hs:hash_vv{V.size_of hs = merkle_tree_size_lg} ->
+  hs:hash_vv #hsz {V.size_of hs = merkle_tree_size_lg} ->
   i:index_t -> j:index_t{j >= i} ->
   p:loc -> h0:HS.mem -> h1:HS.mem ->
   Lemma (requires (V.live h0 hs /\
-                  mt_safe_elts h0 lv hs i j /\
+                  mt_safe_elts #hsz h0 lv hs i j /\
                   loc_disjoint p (V.loc_vector_within hs lv (V.size_of hs)) /\
                   modifies p h0 h1))
-        (ensures (mt_safe_elts h1 lv hs i j))
+        (ensures (mt_safe_elts #hsz h1 lv hs i j))
         (decreases (32 - U32.v lv))
         [SMTPat (V.live h0 hs);
-        SMTPat (mt_safe_elts h0 lv hs i j);
+        SMTPat (mt_safe_elts #hsz h0 lv hs i j);
         SMTPat (loc_disjoint p (RV.loc_rvector hs));
         SMTPat (modifies p h0 h1)]
-let rec mt_safe_elts_preserved lv hs i j p h0 h1 =
+#push-options "--z3rlimit 100 --initial_fuel 2 --max_fuel 2"
+let rec mt_safe_elts_preserved #hsz lv hs i j p h0 h1 =
   if lv = merkle_tree_size_lg then ()
   else (V.get_preserved hs lv p h0 h1;
-       mt_safe_elts_preserved (lv + 1ul) hs (i / 2ul) (j / 2ul) p h0 h1)
+       mt_safe_elts_preserved #hsz (lv + 1ul) hs (i / 2ul) (j / 2ul) p h0 h1)
+#pop-options
 
 // `mt_safe` is the invariant of a Merkle tree through its lifetime.
 // It includes liveness, regionality, disjointness (to each data structure),
@@ -585,8 +583,7 @@ let mt_safe h mt =
 // Since a Merkle tree satisfies regionality, it's ok to take all regions from
 // a tree pointer as a location of the tree.
 val mt_loc: mt_p -> GTot loc
-let mt_loc mt =
-  B.loc_all_regions_from false (B.frameOf mt)
+let mt_loc mt = B.loc_all_regions_from false (B.frameOf mt)
 
 val mt_safe_preserved:
   mt:mt_p -> p:loc -> h0:HS.mem -> h1:HS.mem ->
@@ -612,19 +609,20 @@ let mt_safe_preserved mt p h0 h1 =
 /// Lifting to a high-level Merkle tree structure
 
 val mt_safe_elts_spec:
+  #hsz:hash_size_t ->
   h:HS.mem ->
   lv:uint32_t{lv <= merkle_tree_size_lg} ->
-  hs:hash_vv{V.size_of hs = merkle_tree_size_lg} ->
+  hs:hash_vv #hsz {V.size_of hs = merkle_tree_size_lg} ->
   i:index_t ->
   j:index_t{j >= i} ->
   Lemma (requires (RV.rv_inv h hs /\
                   mt_safe_elts h lv hs i j))
-        (ensures (High.hs_wf_elts
+        (ensures (MTH.hs_wf_elts
                    (U32.v lv) (RV.as_seq h hs)
                    (U32.v i) (U32.v j)))
         (decreases (32 - U32.v lv))
-#push-options "--initial_fuel 2 --max_fuel 2 --initial_ifuel 0 --max_ifuel 0 --z3rlimit 100"
-let rec mt_safe_elts_spec h lv hs i j =
+#push-options "--z3rlimit 100 --initial_fuel 2 --max_fuel 2"
+let rec mt_safe_elts_spec #_ h lv hs i j =
   if lv = merkle_tree_size_lg then ()
   else mt_safe_elts_spec h (lv + 1ul) hs (i / 2ul) (j / 2ul)
 #pop-options
@@ -635,21 +633,22 @@ val merkle_tree_lift:
     RV.rv_inv h (MT?.hs mtv) /\
     RV.rv_inv h (MT?.rhs mtv) /\
     Rgl?.r_inv hreg h (MT?.mroot mtv) /\
-    mt_safe_elts h 0ul (MT?.hs mtv) (MT?.i mtv) (MT?.j mtv)} ->
-  GTot (r:High.merkle_tree{High.mt_wf_elts r})
+    mt_safe_elts #(MT?.hash_size mtv) h 0ul (MT?.hs mtv) (MT?.i mtv) (MT?.j mtv)} ->
+  GTot (r:MTH.merkle_tree #(U32.v (MT?.hash_size mtv)) {MTH.mt_wf_elts #_ r})
 let merkle_tree_lift h mtv =
   mt_safe_elts_spec h 0ul (MT?.hs mtv) (MT?.i mtv) (MT?.j mtv);
-  High.MT
+  MTH.MT #(U32.v (MT?.hash_size mtv))
     (U32.v (MT?.i mtv))
     (U32.v (MT?.j mtv))
     (RV.as_seq h (MT?.hs mtv))
     (MT?.rhs_ok mtv)
     (RV.as_seq h (MT?.rhs mtv))
     (Rgl?.r_repr hreg h (MT?.mroot mtv))
+    (Ghost.reveal (MT?.hash_spec mtv))
 
 val mt_lift:
   h:HS.mem -> mt:mt_p{mt_safe h mt} ->
-  GTot (r:High.merkle_tree{High.mt_wf_elts r})
+  GTot (r:MTH.merkle_tree #(U32.v (MT?.hash_size (B.get h mt 0))) {MTH.mt_wf_elts #_ r})
 let mt_lift h mt =
   merkle_tree_lift h (B.get h mt 0)
 
@@ -679,21 +678,27 @@ let mt_preserved mt p h0 h1 =
 
 // Note that the public function for creation is `mt_create` defined below,
 // which builds a tree with an initial hash.
+#push-options "--z3rlimit 100 --initial_fuel 1 --max_fuel 1 --initial_ifuel 1 --max_ifuel 1"
 private
-val create_empty_mt: r:HST.erid -> hash_fun:hash_fun_t ->
+val create_empty_mt: 
+  #hash_size:hash_size_t -> 
+  #hash_spec:Ghost.erased (MTS.hash_fun_t #(U32.v hash_size)) -> 
+  hash_fun:hash_fun_t #hash_size #hash_spec ->
+  r:HST.erid -> 
   HST.ST mt_p
    (requires (fun _ -> true))
    (ensures (fun h0 mt h1 ->
+     let dmt = B.get h1 mt 0 in
      // memory safety
      B.frameOf mt = r /\
      modifies (mt_loc mt) h0 h1 /\
      mt_safe h1 mt /\
      mt_not_full h1 mt /\
      // correctness
-     mt_lift h1 mt == High.create_empty_mt () /\
-     (MT?.offset (B.get h1 mt 0) = 0UL)))
-#reset-options "--z3rlimit 100"
-let create_empty_mt r hash_fun =
+     MT?.hash_size dmt = hash_size /\
+     MT?.offset dmt = 0UL /\
+     merkle_tree_lift h1 dmt == MTH.create_empty_mt #_ #(Ghost.reveal hash_spec) ()))
+let create_empty_mt #hsz #hash_spec hash_fun r =
   let hs_region = HST.new_region r in
   let hs = RV.alloc_rid hvreg merkle_tree_size_lg hs_region in
   let h0 = HST.get () in
@@ -702,7 +707,7 @@ let create_empty_mt r hash_fun =
   let rhs_region = HST.new_region r in
   let rhs = RV.alloc_rid hreg merkle_tree_size_lg rhs_region in
   let h1 = HST.get () in
-  assert (RV.as_seq h1 rhs == S.create 32 High.hash_init);
+  assert (RV.as_seq h1 rhs == S.create 32 (MTH.hash_init #(U32.v hsz)));
   RV.rv_inv_preserved hs (V.loc_vector rhs) h0 h1;
   RV.as_seq_preserved hs (V.loc_vector rhs) h0 h1;
   V.loc_vector_within_included hs 0ul (V.size_of hs);
@@ -714,13 +719,14 @@ let create_empty_mt r hash_fun =
   RV.as_seq_preserved hs loc_none h1 h2;
   RV.as_seq_preserved rhs loc_none h1 h2;
   mt_safe_elts_preserved 0ul hs 0ul 0ul loc_none h1 h2;
-  let mt = B.malloc r (MT 0UL 0ul 0ul hs false rhs mroot hash_fun) 1ul in
+  let mt = B.malloc r (MT hsz 0UL 0ul 0ul hs false rhs mroot hash_spec hash_fun) 1ul in
   let h3 = HST.get () in
   RV.as_seq_preserved hs loc_none h2 h3;
   RV.as_seq_preserved rhs loc_none h2 h3;
   Rgl?.r_sep hreg mroot loc_none h2 h3;
   mt_safe_elts_preserved 0ul hs 0ul 0ul loc_none h2 h3;
   mt
+#pop-options
 
 /// Destruction (free)
 
@@ -728,13 +734,14 @@ val mt_free: mt:mt_p ->
   HST.ST unit
    (requires (fun h0 -> mt_safe h0 mt))
    (ensures (fun h0 _ h1 -> modifies (mt_loc mt) h0 h1))
-#reset-options "--z3rlimit 100 --max_fuel 0"
+#push-options "--z3rlimit 100"
 let mt_free mt =
   let mtv = !*mt in
   RV.free (MT?.hs mtv);
   RV.free (MT?.rhs mtv);
   Rgl?.r_free hreg (MT?.mroot mtv);
   B.free mt
+#pop-options
 
 /// Insertion
 
@@ -748,7 +755,7 @@ val as_seq_sub_upd:
                           (S.append
                             (RV.as_seq_sub h rv 0ul i)
                             (S.cons v (RV.as_seq_sub h rv (i + 1ul) (V.size_of rv))))))
-#reset-options "--z3rlimit 20"
+#push-options "--z3rlimit 20"
 let as_seq_sub_upd #a #rg h rv i v =
   Seq.Properties.slice_upd (RV.as_seq h rv) 0 (U32.v i) (U32.v i) v;
   Seq.Properties.slice_upd (RV.as_seq h rv) (U32.v i + 1) (U32.v (V.size_of rv)) (U32.v i) v;
@@ -761,27 +768,29 @@ let as_seq_sub_upd #a #rg h rv i v =
   assert (S.equal (S.slice (RV.as_seq h rv) (U32.v i + 1) (U32.v (V.size_of rv)))
                   (RV.as_seq_sub h rv (i + 1ul) (V.size_of rv)));
   assert (S.index (S.upd (RV.as_seq h rv) (U32.v i) v) (U32.v i) == v)
+#pop-options
 
 // `hash_vv_insert_copy` inserts a hash element at a level `lv`, by copying
 // and pushing its content to `hs[lv]`. For detailed insertion procedure, see
 // `insert_` and `mt_insert`.
-#reset-options "--z3rlimit 40"
+#push-options "--z3rlimit 40 --initial_fuel 1 --max_fuel 1"
 inline_for_extraction private
 val hash_vv_insert_copy:
+  #hsz:hash_size_t ->
   lv:uint32_t{lv < merkle_tree_size_lg} ->
   i:Ghost.erased index_t ->
   j:index_t{
     Ghost.reveal i <= j &&
     U32.v j < pow2 (32 - U32.v lv) - 1 &&
     j < uint32_32_max} ->
-  hs:hash_vv{V.size_of hs = merkle_tree_size_lg} ->
-  v:hash ->
+  hs:hash_vv #hsz {V.size_of hs = merkle_tree_size_lg} ->
+  v:hash #hsz ->
   HST.ST unit
     (requires (fun h0 ->
       RV.rv_inv h0 hs /\
       Rgl?.r_inv hreg h0 v /\
       HH.disjoint (V.frameOf hs) (B.frameOf v) /\
-      mt_safe_elts h0 lv hs (Ghost.reveal i) j))
+      mt_safe_elts #hsz h0 lv hs (Ghost.reveal i) j))
     (ensures (fun h0 _ h1 ->
       // memory safety
       modifies (loc_union
@@ -792,20 +801,21 @@ val hash_vv_insert_copy:
       Rgl?.r_inv hreg h1 v /\
       V.size_of (V.get h1 hs lv) == j + 1ul - offset_of (Ghost.reveal i) /\
       V.size_of (V.get h1 hs lv) == V.size_of (V.get h0 hs lv) + 1ul /\
-      mt_safe_elts h1 (lv + 1ul) hs (Ghost.reveal i / 2ul) (j / 2ul) /\
+      mt_safe_elts #hsz h1 (lv + 1ul) hs (Ghost.reveal i / 2ul) (j / 2ul) /\
       RV.rv_loc_elems h0 hs (lv + 1ul) (V.size_of hs) ==
       RV.rv_loc_elems h1 hs (lv + 1ul) (V.size_of hs) /\
       // correctness
-      (mt_safe_elts_spec h0 lv hs (Ghost.reveal i) j;
+      (mt_safe_elts_spec #hsz h0 lv hs (Ghost.reveal i) j;
       S.equal (RV.as_seq h1 hs)
-      (High.hash_ss_insert
+      (MTH.hashess_insert
         (U32.v lv) (U32.v (Ghost.reveal i)) (U32.v j)
         (RV.as_seq h0 hs) (Rgl?.r_repr hreg h0 v))) /\
       S.equal (S.index (RV.as_seq h1 hs) (U32.v lv))
       (S.snoc (S.index (RV.as_seq h0 hs) (U32.v lv))
       (Rgl?.r_repr hreg h0 v))))
-#reset-options "--z3rlimit 100"
-let hash_vv_insert_copy lv i j hs v =
+#pop-options
+#push-options "--z3rlimit 100 --initial_fuel 1 --max_fuel 1"
+let hash_vv_insert_copy #_ lv i j hs v =
   let hh0 = HST.get () in
   mt_safe_elts_rec hh0 lv hs (Ghost.reveal i) j;
 
@@ -903,6 +913,7 @@ let hash_vv_insert_copy lv i j hs v =
                     (S.cons (RV.as_seq hh1 ihv)
                             (RV.as_seq_sub hh0 hs (lv + 1ul) merkle_tree_size_lg))));
   as_seq_sub_upd hh0 hs lv (RV.as_seq hh1 ihv)
+#pop-options
 
 private
 val insert_index_helper_even:
@@ -912,6 +923,7 @@ val insert_index_helper_even:
         (ensures (U32.v j % 2 <> 1 /\ j / 2ul == (j + 1ul) / 2ul))
 let insert_index_helper_even lv j = ()
 
+#push-options "--z3rlimit 100 --initial_fuel 1 --max_fuel 1 --initial_ifuel 1 --max_ifuel 1"
 private
 val insert_index_helper_odd:
   lv:uint32_t{lv < merkle_tree_size_lg} ->
@@ -924,6 +936,7 @@ val insert_index_helper_odd:
                  (j + 1ul) / 2ul == j / 2ul + 1ul /\
                  j - offset_of i > 0ul))
 let insert_index_helper_odd lv i j = ()
+#pop-options
 
 private
 val loc_union_assoc_4:
@@ -938,8 +951,9 @@ let loc_union_assoc_4 a b c d =
 
 private
 val insert_modifies_rec_helper:
+  #hsz:hash_size_t ->
   lv:uint32_t{lv < merkle_tree_size_lg} ->
-  hs:hash_vv{V.size_of hs = merkle_tree_size_lg} ->
+  hs:hash_vv #hsz {V.size_of hs = merkle_tree_size_lg} ->
   aloc:loc ->
   h:HS.mem ->
   Lemma (loc_union
@@ -958,7 +972,8 @@ val insert_modifies_rec_helper:
               (RV.rv_loc_elems h hs lv (V.size_of hs))
               (V.loc_vector_within hs lv (V.size_of hs)))
             aloc)
-let insert_modifies_rec_helper lv hs aloc h =
+#push-options "--z3rlimit 100 --initial_fuel 2 --max_fuel 2"
+let insert_modifies_rec_helper #hsz lv hs aloc h =
   assert (V.loc_vector_within hs lv (V.size_of hs) ==
          loc_union (V.loc_vector_within hs lv (lv + 1ul))
                    (V.loc_vector_within hs (lv + 1ul) (V.size_of hs)));
@@ -994,6 +1009,7 @@ let insert_modifies_rec_helper lv hs aloc h =
     (V.loc_vector_within hs lv (lv + 1ul))
     (RV.rv_loc_elems h hs (lv + 1ul) (V.size_of hs))
     (V.loc_vector_within hs (lv + 1ul) (V.size_of hs))
+#pop-options
 
 private
 val insert_modifies_union_loc_weakening:
@@ -1032,15 +1048,17 @@ let rv_inv_rv_elems_reg #a #rg h rv i j = ()
 //
 private
 val insert_:
+  #hsz:hash_size_t ->
+  #hash_spec:Ghost.erased (MTS.hash_fun_t #(U32.v hsz)) ->
   lv:uint32_t{lv < merkle_tree_size_lg} ->
   i:Ghost.erased index_t ->
   j:index_t{
     Ghost.reveal i <= j &&
     U32.v j < pow2 (32 - U32.v lv) - 1 &&
     j < uint32_32_max} ->
-  hs:hash_vv{V.size_of hs = merkle_tree_size_lg} ->
-  acc:hash ->
-  hash_fun:hash_fun_t ->
+  hs:hash_vv #hsz {V.size_of hs = merkle_tree_size_lg} ->
+  acc:hash #hsz ->
+  hash_fun:hash_fun_t #hsz #hash_spec ->
   HST.ST unit
          (requires (fun h0 ->
            RV.rv_inv h0 hs /\
@@ -1061,11 +1079,11 @@ val insert_:
            // correctness
            (mt_safe_elts_spec h0 lv hs (Ghost.reveal i) j;
            S.equal (RV.as_seq h1 hs)
-                   (High.insert_ (U32.v lv) (U32.v (Ghost.reveal i)) (U32.v j)
+                   (MTH.insert_ #(U32.v hsz) #hash_spec (U32.v lv) (U32.v (Ghost.reveal i)) (U32.v j)
                      (RV.as_seq h0 hs) (Rgl?.r_repr hreg h0 acc)))))
          (decreases (U32.v j))
-#reset-options "--z3rlimit 800 --max_fuel 1"
-let rec insert_ lv i j hs acc hash_fun =
+#push-options "--z3rlimit 800 --initial_fuel 2 --max_fuel 2 --initial_ifuel 2 --max_ifuel 2"
+let rec insert_ #hsz #hash_spec lv i j hs acc hash_fun =
   let hh0 = HST.get () in
   hash_vv_insert_copy lv i j hs acc;
   let hh1 = HST.get () in
@@ -1124,8 +1142,8 @@ let rec insert_ lv i j hs acc hash_fun =
        insert_snoc_last_helper
          (RV.as_seq hh0 (V.get hh0 hs lv))
          (Rgl?.r_repr hreg hh0 acc);
-       assert (S.equal (Rgl?.r_repr hreg hh2 acc) // `nacc` in `High.insert_`
-                       (High.hash_2
+       assert (S.equal (Rgl?.r_repr hreg hh2 acc) // `nacc` in `MTH.insert_`
+                       (MTH.sha256_compress
                          (S.last (S.index (RV.as_seq hh0 hs) (U32.v lv)))
                          (Rgl?.r_repr hreg hh0 acc)));
 
@@ -1185,13 +1203,13 @@ let rec insert_ lv i j hs acc hash_fun =
        // 4-2) Correctness
        mt_safe_elts_spec hh2 (lv + 1ul) hs (Ghost.reveal i / 2ul) (j / 2ul);
        assert (S.equal (RV.as_seq hh3 hs)
-       (High.insert_ (U32.v lv + 1) (U32.v (Ghost.reveal i) / 2) (U32.v j / 2)
+       (MTH.insert_ #(U32.v hsz) #(Ghost.reveal hash_spec) (U32.v lv + 1) (U32.v (Ghost.reveal i) / 2) (U32.v j / 2)
          (RV.as_seq hh2 hs) (Rgl?.r_repr hreg hh2 acc)));
        mt_safe_elts_spec hh0 lv hs (Ghost.reveal i) j;
-       High.insert_rec (U32.v lv) (U32.v (Ghost.reveal i)) (U32.v j)
+       MTH.insert_rec #(U32.v hsz) #(Ghost.reveal hash_spec) (U32.v lv) (U32.v (Ghost.reveal i)) (U32.v j)
          (RV.as_seq hh0 hs) (Rgl?.r_repr hreg hh0 acc);
        assert (S.equal (RV.as_seq hh3 hs)
-       (High.insert_ (U32.v lv) (U32.v (Ghost.reveal i)) (U32.v j)
+       (MTH.insert_ #(U32.v hsz) #(Ghost.reveal hash_spec) (U32.v lv) (U32.v (Ghost.reveal i)) (U32.v j)
          (RV.as_seq hh0 hs) (Rgl?.r_repr hreg hh0 acc))))
   else (insert_index_helper_even lv j;
        // memory safety
@@ -1216,10 +1234,10 @@ let rec insert_ lv i j hs acc hash_fun =
          hh0 hh1;
        // correctness
        mt_safe_elts_spec hh0 lv hs (Ghost.reveal i) j;
-       High.insert_base (U32.v lv) (U32.v (Ghost.reveal i)) (U32.v j)
+       MTH.insert_base #(U32.v hsz) #(Ghost.reveal hash_spec) (U32.v lv) (U32.v (Ghost.reveal i)) (U32.v j)
          (RV.as_seq hh0 hs) (Rgl?.r_repr hreg hh0 acc);
        assert (S.equal (RV.as_seq hh1 hs)
-              (High.insert_ (U32.v lv) (U32.v (Ghost.reveal i)) (U32.v j)
+              (MTH.insert_ #(U32.v hsz) #(Ghost.reveal hash_spec) (U32.v lv) (U32.v (Ghost.reveal i)) (U32.v j)
                 (RV.as_seq hh0 hs) (Rgl?.r_repr hreg hh0 acc))));
 
   /// 5) Proving the postcondition after recursion
@@ -1252,32 +1270,37 @@ let rec insert_ lv i j hs acc hash_fun =
   // 5-4) Correctness
   mt_safe_elts_spec hh0 lv hs (Ghost.reveal i) j;
   assert (S.equal (RV.as_seq hh4 hs)
-                  (High.insert_ (U32.v lv) (U32.v (Ghost.reveal i)) (U32.v j)
+                  (MTH.insert_ #(U32.v hsz) #hash_spec (U32.v lv) (U32.v (Ghost.reveal i)) (U32.v j)
                     (RV.as_seq hh0 hs) (Rgl?.r_repr hreg hh0 acc))) // QED
-#reset-options
+#pop-options
 
 private inline_for_extraction
-val mt_insert_pre_nst: mtv:merkle_tree -> v:hash -> Tot bool
+val mt_insert_pre_nst: mtv:merkle_tree -> v:hash #(MT?.hash_size mtv) -> Tot bool
 let mt_insert_pre_nst mtv v = mt_not_full_nst mtv && add64_fits (MT?.offset mtv) ((MT?.j mtv) + 1ul)
 
-val mt_insert_pre: mt:const_mt_p -> v:hash -> HST.ST bool
-  (requires (fun h0 -> mt_safe h0 (CB.cast mt)))
+val mt_insert_pre: #hsz:hash_size_t -> mt:const_mt_p -> v:hash #hsz -> HST.ST bool
+  (requires (fun h0 -> mt_safe h0 (CB.cast mt) /\ (MT?.hash_size (B.get h0 (CB.cast mt) 0)) = hsz))
   (ensures (fun _ _ _ -> True))
-let mt_insert_pre mt v = 
+let mt_insert_pre #hsz mt v = 
   let mt = CB.cast mt in
-  mt_insert_pre_nst !*mt v
+  let mt = !*mt in
+  assert (MT?.hash_size mt == hsz);
+  mt_insert_pre_nst mt v
 
 // `mt_insert` inserts a hash to a Merkle tree. Note that this operation
 // manipulates the content in `v`, since it uses `v` as an accumulator during
 // insertion.
 val mt_insert:
-  mt:mt_p -> v:hash ->
+  #hsz:hash_size_t ->
+  mt:mt_p -> v:hash #hsz ->
   HST.ST unit
    (requires (fun h0 ->
+     let dmt = B.get h0 mt 0 in
      mt_safe h0 mt /\
      Rgl?.r_inv hreg h0 v /\
      HH.disjoint (B.frameOf mt) (B.frameOf v) /\
-     mt_insert_pre_nst (B.get h0 mt 0) v))
+     MT?.hash_size dmt = hsz /\
+     mt_insert_pre_nst dmt v))
    (ensures (fun h0 _ h1 ->
      // memory safety
      modifies (loc_union
@@ -1286,13 +1309,14 @@ val mt_insert:
               h0 h1 /\
      mt_safe h1 mt /\
      // correctness
-     mt_lift h1 mt == High.mt_insert (mt_lift h0 mt) (Rgl?.r_repr hreg h0 v)))
-#reset-options "--z3rlimit 40 --max_fuel 0"
-let mt_insert mt v =
+     MT?.hash_size (B.get h1 mt 0) = hsz /\
+     mt_lift h1 mt == MTH.mt_insert (mt_lift h0 mt) (Rgl?.r_repr hreg h0 v)))
+#push-options "--z3rlimit 40"
+let mt_insert #hsz mt v =
   let hh0 = HST.get () in
   let mtv = !*mt in
   let hs = MT?.hs mtv in
-  insert_ 0ul (Ghost.hide (MT?.i mtv)) (MT?.j mtv) hs v (MT?.hash_fun mtv);
+  insert_ #hsz #(Ghost.reveal (MT?.hash_spec mtv)) 0ul (Ghost.hide (MT?.i mtv)) (MT?.j mtv) hs v (MT?.hash_fun mtv);
   let hh1 = HST.get () in
   RV.rv_loc_elems_included hh0 (MT?.hs mtv) 0ul (V.size_of hs);
   V.loc_vector_within_included hs 0ul (V.size_of hs);
@@ -1319,13 +1343,15 @@ let mt_insert mt v =
         (V.loc_vector_within hs 0ul (V.size_of hs)))
       (B.loc_all_regions_from false (B.frameOf v)))
     hh0 hh1;
-  mt *= MT (MT?.offset mtv)
+  mt *= MT (MT?.hash_size mtv) 
+           (MT?.offset mtv)
            (MT?.i mtv)
            (MT?.j mtv + 1ul)
            (MT?.hs mtv)
            false // `rhs` is always deprecated right after an insertion.
            (MT?.rhs mtv)
            (MT?.mroot mtv)
+           (MT?.hash_spec mtv)
            (MT?.hash_fun mtv);
   let hh2 = HST.get () in
   RV.rv_inv_preserved
@@ -1340,11 +1366,14 @@ let mt_insert mt v =
   mt_safe_elts_preserved
     0ul (MT?.hs mtv) (MT?.i mtv) (MT?.j mtv + 1ul) (B.loc_buffer mt)
     hh1 hh2
-#reset-options // reset "--max_fuel 0"
+#pop-options
 
 // `mt_create` initiates a Merkle tree with a given initial hash `init`.
 // A valid Merkle tree should contain at least one element.
-val mt_create_custom: r:HST.erid -> init:hash -> hash_fun:hash_fun_t -> HST.ST mt_p
+val mt_create_custom: 
+  #hsz:hash_size_t -> 
+  #hash_spec:Ghost.erased (MTS.hash_fun_t #(U32.v hsz)) ->
+  r:HST.erid -> init:hash #hsz -> hash_fun:hash_fun_t #hsz #hash_spec -> HST.ST mt_p
    (requires (fun h0 ->
      Rgl?.r_inv hreg h0 init /\
      HH.disjoint r (B.frameOf init)))
@@ -1353,16 +1382,18 @@ val mt_create_custom: r:HST.erid -> init:hash -> hash_fun:hash_fun_t -> HST.ST m
      modifies (loc_union (mt_loc mt) (B.loc_all_regions_from false (B.frameOf init))) h0 h1 /\
      mt_safe h1 mt /\
      // correctness
-     mt_lift h1 mt == High.create_mt (Rgl?.r_repr hreg h0 init)))
-#reset-options "--z3rlimit 40"
-let mt_create_custom r init hash_fun =
+     MT?.hash_size (B.get h1 mt 0) = hsz /\     
+     mt_lift h1 mt == MTH.mt_create (U32.v hsz) (Ghost.reveal hash_spec) (Rgl?.r_repr hreg h0 init)))
+#push-options "--z3rlimit 40"
+let mt_create_custom #hsz #hash_spec r init hash_fun =
   let hh0 = HST.get () in
-  let mt = create_empty_mt r hash_fun in
+  let mt = create_empty_mt #hsz #hash_spec hash_fun r in
   mt_insert mt init;
   let hh2 = HST.get () in
   mt
+#pop-options
 
-val mt_create: r:HST.erid -> init:hash -> HST.ST mt_p
+val mt_create: r:HST.erid -> init:hash #32ul -> HST.ST mt_p
    (requires (fun h0 ->
      Rgl?.r_inv hreg h0 init /\
      HH.disjoint r (B.frameOf init)))
@@ -1371,8 +1402,9 @@ val mt_create: r:HST.erid -> init:hash -> HST.ST mt_p
      modifies (loc_union (mt_loc mt) (B.loc_all_regions_from false (B.frameOf init))) h0 h1 /\
      mt_safe h1 mt /\
      // correctness
-     mt_lift h1 mt == High.create_mt (Rgl?.r_repr hreg h0 init)))
-let mt_create r init = mt_create_custom r init hash_2
+     MT?.hash_size (B.get h1 mt 0) = 32ul /\
+     mt_lift h1 mt == MTH.mt_create 32 MTH.sha256_compress (Rgl?.r_repr hreg h0 init)))
+let mt_create r init = mt_create_custom #32ul #(Ghost.hide MTH.sha256_compress) r init sha256_compress
 
 /// Construction and Destruction of paths
 
@@ -1380,14 +1412,15 @@ let mt_create r init = mt_create_custom r init hash_2
 // each element has different location in `MT?.hs` (thus different region id),
 // we cannot use the regionality property for `path`s. Hence here we manually
 // define invariants and representation.
-type path = V.vector hash
-type path_p = B.pointer path
-type const_path_p = const_pointer path
+type path (#hsz:hash_size_t) = V.vector (hash #hsz)
+type path_p (#hsz:hash_size_t) = B.pointer (path #hsz)
+type const_path_p (#hsz:hash_size_t) = const_pointer (path #hsz)
 
 // Memory safety of a path as an invariant
 val path_safe:
-  HS.mem -> mtr:HH.rid -> path_p -> GTot Type0
-let path_safe h mtr p =
+  #hsz:hash_size_t ->
+  HS.mem -> mtr:HH.rid -> path_p #hsz -> GTot Type0
+let path_safe #_ h mtr p =
   B.live h p /\ B.freeable p /\
   V.live h (B.get h p 0) /\ V.freeable (B.get h p 0) /\
   HST.is_eternal_region (V.frameOf (B.get h p 0)) /\
@@ -1397,34 +1430,36 @@ let path_safe h mtr p =
   HH.extends (V.frameOf (B.get h p 0)) (B.frameOf p) /\
   HH.disjoint mtr (B.frameOf p)
 
-val path_loc: path_p -> GTot loc
-let path_loc p =
-  B.loc_all_regions_from false (B.frameOf p)
+val path_loc: #hsz:hash_size_t -> path_p #hsz -> GTot loc
+let path_loc #_ p = B.loc_all_regions_from false (B.frameOf p)
 
 val lift_path_:
+  #hsz:hash_size_t ->
   h:HS.mem ->
-  hs:S.seq hash ->
+  hs:S.seq (hash #hsz) ->
   i:nat ->
   j:nat{
     i <= j /\ j <= S.length hs /\
     V.forall_seq hs i j (fun hp -> Rgl?.r_inv hreg h hp)} ->
-  GTot (hp:High.path{S.length hp = j - i}) (decreases j)
-let rec lift_path_ h hs i j =
+  GTot (hp:MTH.path #(U32.v hsz) {S.length hp = j - i}) (decreases j)
+let rec lift_path_ #_ h hs i j =
   if i = j then S.empty
   else (S.snoc (lift_path_ h hs i (j - 1))
                (Rgl?.r_repr hreg h (S.index hs (j - 1))))
 
 // Representation of a path
 val lift_path:
-  h:HS.mem -> mtr:HH.rid -> p:path_p{path_safe h mtr p} ->
-  GTot (hp:High.path{S.length hp = U32.v (V.size_of (B.get h p 0))})
-let lift_path h mtr p =
+  #hsz:hash_size_t ->
+  h:HS.mem -> mtr:HH.rid -> p:path_p #hsz {path_safe h mtr p} ->
+  GTot (hp:MTH.path #(U32.v hsz) {S.length hp = U32.v (V.size_of (B.get h p 0))})
+let lift_path #_ h mtr p =
   lift_path_ h (V.as_seq h (B.get h p 0))
     0 (S.length (V.as_seq h (B.get h p 0)))
 
 val lift_path_index_:
+  #hsz:hash_size_t ->
   h:HS.mem ->
-  hs:S.seq hash ->
+  hs:S.seq (hash #hsz) ->
   i:nat -> j:nat{i <= j && j <= S.length hs} ->
   k:nat{i <= k && k < j} ->
   Lemma (requires (V.forall_seq hs i j (fun hp -> Rgl?.r_inv hreg h hp)))
@@ -1432,32 +1467,36 @@ val lift_path_index_:
                  S.index (lift_path_ h hs i j) (k - i)))
         (decreases j)
         [SMTPat (S.index (lift_path_ h hs i j) (k - i))]
-let rec lift_path_index_ h hs i j k =
+#push-options "--initial_fuel 1 --max_fuel 1 --initial_ifuel 1 --max_ifuel 1"
+let rec lift_path_index_ #hsz h hs i j k =
   if i = j then ()
   else if k = j - 1 then ()
-  else lift_path_index_ h hs i (j - 1) k
+  else lift_path_index_ #hsz h hs i (j - 1) k
+#pop-options
 
 val lift_path_index:
+  #hsz:hash_size_t ->
   h:HS.mem -> mtr:HH.rid ->
-  p:path_p -> i:uint32_t ->
+  p:path_p #hsz -> i:uint32_t ->
   Lemma (requires (path_safe h mtr p /\
                   i < V.size_of (B.get h p 0)))
         (ensures (Rgl?.r_repr hreg h (V.get h (B.get h p 0) i) ==
                  S.index (lift_path h mtr p) (U32.v i)))
-let lift_path_index h mtr p i =
+let lift_path_index #_ h mtr p i =
   lift_path_index_ h (V.as_seq h (B.get h p 0))
     0 (S.length (V.as_seq h (B.get h p 0))) (U32.v i)
 
 val lift_path_eq:
+  #hsz:hash_size_t ->
   h:HS.mem ->
-  hs1:S.seq hash -> hs2:S.seq hash ->
+  hs1:S.seq (hash #hsz) -> hs2:S.seq (hash #hsz) ->
   i:nat -> j:nat ->
   Lemma (requires (i <= j /\ j <= S.length hs1 /\ j <= S.length hs2 /\
                   S.equal (S.slice hs1 i j) (S.slice hs2 i j) /\
                   V.forall_seq hs1 i j (fun hp -> Rgl?.r_inv hreg h hp) /\
                   V.forall_seq hs2 i j (fun hp -> Rgl?.r_inv hreg h hp)))
         (ensures (S.equal (lift_path_ h hs1 i j) (lift_path_ h hs2 i j)))
-let lift_path_eq h hs1 hs2 i j =
+let lift_path_eq #_ h hs1 hs2 i j =
   assert (forall (k:nat{i <= k && k < j}).
            S.index (lift_path_ h hs1 i j) (k - i) ==
            Rgl?.r_repr hreg h (S.index hs1 k));
@@ -1477,7 +1516,8 @@ let lift_path_eq h hs1 hs2 i j =
 
 private
 val path_safe_preserved_:
-  mtr:HH.rid -> hs:S.seq hash ->
+  #hsz:hash_size_t ->
+  mtr:HH.rid -> hs:S.seq (hash #hsz) ->
   i:nat -> j:nat{i <= j && j <= S.length hs} ->
   dl:loc -> h0:HS.mem -> h1:HS.mem ->
   Lemma
@@ -1492,7 +1532,7 @@ val path_safe_preserved_:
                  Rgl?.r_inv hreg h1 hp /\
                  HH.includes mtr (Rgl?.region_of hreg hp))))
     (decreases j)
-let rec path_safe_preserved_ mtr hs i j dl h0 h1 =
+let rec path_safe_preserved_ #_ mtr hs i j dl h0 h1 =
   if i = j then ()
   else (assert (loc_includes
                  (B.loc_all_regions_from false mtr)
@@ -1502,14 +1542,15 @@ let rec path_safe_preserved_ mtr hs i j dl h0 h1 =
        path_safe_preserved_ mtr hs i (j - 1) dl h0 h1)
 
 val path_safe_preserved:
-  mtr:HH.rid -> p:path_p ->
+  #hsz:hash_size_t ->
+  mtr:HH.rid -> p:path_p #hsz ->
   dl:loc -> h0:HS.mem -> h1:HS.mem ->
   Lemma (requires (path_safe h0 mtr p /\
                   loc_disjoint dl (path_loc p) /\
                   loc_disjoint dl (B.loc_all_regions_from false mtr) /\
                   modifies dl h0 h1))
         (ensures (path_safe h1 mtr p))
-let path_safe_preserved mtr p dl h0 h1 =
+let path_safe_preserved #_ mtr p dl h0 h1 =
   assert (loc_includes (path_loc p) (B.loc_buffer p));
   assert (loc_includes (path_loc p) (V.loc_vector (B.get h0 p 0)));
   path_safe_preserved_
@@ -1517,7 +1558,8 @@ let path_safe_preserved mtr p dl h0 h1 =
     0 (S.length (V.as_seq h0 (B.get h0 p 0))) dl h0 h1
 
 val path_safe_init_preserved:
-  mtr:HH.rid -> p:path_p ->
+  #hsz:hash_size_t ->
+  mtr:HH.rid -> p:path_p #hsz ->
   dl:loc -> h0:HS.mem -> h1:HS.mem ->
   Lemma (requires (path_safe h0 mtr p /\
                   V.size_of (B.get h0 p 0) = 0ul /\
@@ -1525,13 +1567,14 @@ val path_safe_init_preserved:
                   modifies dl h0 h1))
         (ensures (path_safe h1 mtr p /\
                  V.size_of (B.get h1 p 0) = 0ul))
-let path_safe_init_preserved mtr p dl h0 h1 =
+let path_safe_init_preserved #_ mtr p dl h0 h1 =
   assert (loc_includes (path_loc p) (B.loc_buffer p));
   assert (loc_includes (path_loc p) (V.loc_vector (B.get h0 p 0)))
 
 val path_preserved_:
+  #hsz:hash_size_t ->
   mtr:HH.rid ->
-  hs:S.seq hash ->
+  hs:S.seq (hash #hsz) ->
   i:nat -> j:nat{i <= j && j <= S.length hs} ->
   dl:loc -> h0:HS.mem -> h1:HS.mem ->
   Lemma (requires (V.forall_seq hs i j
@@ -1543,7 +1586,8 @@ val path_preserved_:
                  S.equal (lift_path_ h0 hs i j)
                          (lift_path_ h1 hs i j)))
         (decreases j)
-let rec path_preserved_ mtr hs i j dl h0 h1 =
+#push-options "--initial_fuel 1 --max_fuel 1 --initial_ifuel 1 --max_ifuel 1"
+let rec path_preserved_ #_ mtr hs i j dl h0 h1 =
   if i = j then ()
   else (path_safe_preserved_ mtr hs i (j - 1) dl h0 h1;
        path_preserved_ mtr hs i (j - 1) dl h0 h1;
@@ -1552,9 +1596,11 @@ let rec path_preserved_ mtr hs i j dl h0 h1 =
                 (B.loc_all_regions_from false
                   (Rgl?.region_of hreg (S.index hs (j - 1)))));
        Rgl?.r_sep hreg (S.index hs (j - 1)) dl h0 h1)
+#pop-options
 
 val path_preserved:
-  mtr:HH.rid -> p:path_p ->
+  #hsz:hash_size_t ->
+  mtr:HH.rid -> p:path_p #hsz ->
   dl:loc -> h0:HS.mem -> h1:HS.mem ->
   Lemma (requires (path_safe h0 mtr p /\
                   loc_disjoint dl (path_loc p) /\
@@ -1562,7 +1608,7 @@ val path_preserved:
                   modifies dl h0 h1))
         (ensures (path_safe_preserved mtr p dl h0 h1;
                  S.equal (lift_path h0 mtr p) (lift_path h1 mtr p)))
-let path_preserved mtr p dl h0 h1 =
+let path_preserved #_ mtr p dl h0 h1 =
   assert (loc_includes (path_loc p) (B.loc_buffer p));
   assert (loc_includes (path_loc p) (V.loc_vector (B.get h0 p 0)));
   path_preserved_ mtr (V.as_seq h0 (B.get h0 p 0))
@@ -1570,20 +1616,22 @@ let path_preserved mtr p dl h0 h1 =
     dl h0 h1
 
 val init_path:
+  #hsz:hash_size_t ->
   mtr:HH.rid -> r:HST.erid ->
-  HST.ST path_p
+  HST.ST (path_p #hsz)
     (requires (fun h0 -> HH.disjoint mtr r))
     (ensures (fun h0 p h1 ->
       // memory safety
       path_safe h1 mtr p /\
       // correctness
       S.equal (lift_path h1 mtr p) S.empty))
-let init_path mtr r =
+let init_path #_ mtr r =
   let nrid = HST.new_region r in
   B.malloc r (hash_vec_r_alloc nrid) 1ul
 
 val clear_path:
-  mtr:HH.rid -> p:path_p ->
+  #hsz:hash_size_t ->
+  mtr:HH.rid -> p:path_p #hsz ->
   HST.ST unit
     (requires (fun h0 -> path_safe h0 mtr p))
     (ensures (fun h0 _ h1 ->
@@ -1592,11 +1640,12 @@ val clear_path:
       // correctness
       V.size_of (B.get h1 p 0) = 0ul /\
       S.equal (lift_path h1 mtr p) S.empty))
-let clear_path mtr p =
+let clear_path #_ mtr p =
   p *= V.clear !*p
 
 val free_path:
-  p:path_p ->
+  #hsz:hash_size_t ->
+  p:path_p #hsz ->
   HST.ST unit
     (requires (fun h0 ->
       B.live h0 p /\ B.freeable p /\
@@ -1604,7 +1653,7 @@ val free_path:
       HH.extends (V.frameOf (B.get h0 p 0)) (B.frameOf p)))
     (ensures (fun h0 _ h1 ->
       modifies (path_loc p) h0 h1))
-let free_path p =
+let free_path #_ p =
   V.free !*p;
   B.free p
 
@@ -1615,14 +1664,16 @@ let free_path p =
 // accumulator value.
 private
 val construct_rhs:
+  #hsz:hash_size_t ->
+  #hash_spec:Ghost.erased (MTS.hash_fun_t #(U32.v hsz)) ->
   lv:uint32_t{lv <= merkle_tree_size_lg} ->
-  hs:hash_vv{V.size_of hs = merkle_tree_size_lg} ->
-  rhs:hash_vec{V.size_of rhs = merkle_tree_size_lg} ->
+  hs:hash_vv #hsz {V.size_of hs = merkle_tree_size_lg} ->
+  rhs:hash_vec #hsz {V.size_of rhs = merkle_tree_size_lg} ->
   i:index_t ->
   j:index_t{i <= j && U32.v j < pow2 (32 - U32.v lv)} ->
   acc:hash ->
   actd:bool ->
-  hash_fun:hash_fun_t ->
+  hash_fun:hash_fun_t #hsz #(Ghost.reveal hash_spec) ->
   HST.ST unit
    (requires (fun h0 ->
      RV.rv_inv h0 hs /\ RV.rv_inv h0 rhs /\
@@ -1641,16 +1692,16 @@ val construct_rhs:
      Rgl?.r_inv hreg h1 acc /\
      // correctness
      (mt_safe_elts_spec h0 lv hs i j;
-     High.construct_rhs
+     MTH.construct_rhs #(U32.v hsz) #(Ghost.reveal hash_spec)
        (U32.v lv)
        (Rgl?.r_repr hvvreg h0 hs)
        (Rgl?.r_repr hvreg h0 rhs)
        (U32.v i) (U32.v j)
        (Rgl?.r_repr hreg h0 acc) actd ==
-     (Rgl?.r_repr hvreg h1 rhs, Rgl?.r_repr hreg h1 acc))))
+     (Rgl?.r_repr hvreg h1 rhs, Rgl?.r_repr (hreg #hsz) h1 acc))))
    (decreases (U32.v j))
-#reset-options "--z3rlimit 400 --max_fuel 1"
-let rec construct_rhs lv hs rhs i j acc actd hash_fun =
+#push-options "--z3rlimit 400 --initial_fuel 1 --max_fuel 1 --initial_ifuel 1 --max_ifuel 1"
+let rec construct_rhs #hsz #hash_spec lv hs rhs i j acc actd hash_fun =
   let hh0 = HST.get () in
   let ofs = offset_of i in
   let copy = Cpy?.copy hcpy in
@@ -1665,10 +1716,10 @@ let rec construct_rhs lv hs rhs i j acc actd hash_fun =
       let hh1 = HST.get () in
       // correctness
       mt_safe_elts_spec hh0 lv hs i j;
-      High.construct_rhs_even
+      MTH.construct_rhs_even #(U32.v hsz) #(Ghost.reveal hash_spec)
         (U32.v lv) (Rgl?.r_repr hvvreg hh0 hs) (Rgl?.r_repr hvreg hh0 rhs)
         (U32.v i) (U32.v j) (Rgl?.r_repr hreg hh0 acc) actd;
-      assert (High.construct_rhs
+      assert (MTH.construct_rhs #(U32.v hsz) #(Ghost.reveal hash_spec)
                (U32.v lv)
                (Rgl?.r_repr hvvreg hh0 hs)
                (Rgl?.r_repr hvreg hh0 rhs)
@@ -1723,9 +1774,9 @@ let rec construct_rhs lv hs rhs i j acc actd hash_fun =
         // correctness
         hash_vv_as_seq_get_index hh0 hs lv (j - 1ul - ofs);
         assert (Rgl?.r_repr hreg hh2 acc ==
-               High.hash_2 (S.index (S.index (RV.as_seq hh0 hs) (U32.v lv))
-                                    (U32.v j - 1 - U32.v ofs))
-                           (Rgl?.r_repr hreg hh0 acc))
+               (Ghost.reveal hash_spec) (S.index (S.index (RV.as_seq hh0 hs) (U32.v lv))
+                                        (U32.v j - 1 - U32.v ofs))
+               (Rgl?.r_repr hreg hh0 acc))
       end
 
       else begin
@@ -1762,7 +1813,7 @@ let rec construct_rhs lv hs rhs i j acc actd hash_fun =
                       else RV.as_seq hh0 rhs));
       assert (Rgl?.r_repr hreg hh3 acc ==
              (if actd
-             then High.hash_2 (S.index (S.index (RV.as_seq hh0 hs) (U32.v lv))
+             then (Ghost.reveal hash_spec) (S.index (S.index (RV.as_seq hh0 hs) (U32.v lv))
                                        (U32.v j - 1 - U32.v ofs))
                               (Rgl?.r_repr hreg hh0 acc)
              else S.index (S.index (RV.as_seq hh0 hs) (U32.v lv))
@@ -1772,7 +1823,7 @@ let rec construct_rhs lv hs rhs i j acc actd hash_fun =
       construct_rhs (lv + 1ul) hs rhs (i / 2ul) (j / 2ul) acc true hash_fun;
       let hh4 = HST.get () in
       mt_safe_elts_spec hh3 (lv + 1ul) hs (i / 2ul) (j / 2ul);
-      assert (High.construct_rhs
+      assert (MTH.construct_rhs #(U32.v hsz) #(Ghost.reveal hash_spec)
                (U32.v lv + 1)
                (Rgl?.r_repr hvvreg hh3 hs)
                (Rgl?.r_repr hvreg hh3 rhs)
@@ -1780,10 +1831,10 @@ let rec construct_rhs lv hs rhs i j acc actd hash_fun =
                (Rgl?.r_repr hreg hh3 acc) true ==
              (Rgl?.r_repr hvreg hh4 rhs, Rgl?.r_repr hreg hh4 acc));
       mt_safe_elts_spec hh0 lv hs i j;
-      High.construct_rhs_odd
+      MTH.construct_rhs_odd #(U32.v hsz) #(Ghost.reveal hash_spec)
         (U32.v lv) (Rgl?.r_repr hvvreg hh0 hs) (Rgl?.r_repr hvreg hh0 rhs)
         (U32.v i) (U32.v j) (Rgl?.r_repr hreg hh0 acc) actd;
-      assert (High.construct_rhs
+      assert (MTH.construct_rhs #(U32.v hsz) #(Ghost.reveal hash_spec)
                (U32.v lv)
                (Rgl?.r_repr hvvreg hh0 hs)
                (Rgl?.r_repr hvreg hh0 rhs)
@@ -1791,24 +1842,28 @@ let rec construct_rhs lv hs rhs i j acc actd hash_fun =
                (Rgl?.r_repr hreg hh0 acc) actd ==
              (Rgl?.r_repr hvreg hh4 rhs, Rgl?.r_repr hreg hh4 acc))
     end)
-#reset-options
+#pop-options
 
 private inline_for_extraction
-val mt_get_root_pre_nst: mtv:merkle_tree -> rt:hash -> Tot bool
+val mt_get_root_pre_nst: mtv:merkle_tree -> rt:hash #(MT?.hash_size mtv) -> Tot bool
 let mt_get_root_pre_nst mtv rt = true
 
 val mt_get_root_pre:
+  #hsz:hash_size_t ->
   mt:const_mt_p ->
-  rt:hash ->
+  rt:hash #hsz ->
   HST.ST bool
    (requires (fun h0 ->
      let mt = CB.cast mt in
+     MT?.hash_size (B.get h0 mt 0) = hsz /\
      mt_safe h0 mt /\ Rgl?.r_inv hreg h0 rt /\
      HH.disjoint (B.frameOf mt) (B.frameOf rt)))
    (ensures (fun _ _ _ -> True))
-let mt_get_root_pre mt rt = 
+let mt_get_root_pre #hsz mt rt = 
   let mt = CB.cast mt in
-  mt_get_root_pre_nst !*mt rt
+  let mt = !*mt in
+  assert (MT?.hash_size mt = hsz);
+  mt_get_root_pre_nst mt rt
 
 // `mt_get_root` returns the Merkle root. If it's already calculated with
 // up-to-date hashes, the root is returned immediately. Otherwise it calls
@@ -1839,7 +1894,7 @@ val mt_get_root:
      MT?.rhs_ok mtv1 = true /\
      Rgl?.r_inv hreg h1 rt /\
      // correctness
-     High.mt_get_root (mt_lift h0 mt) (Rgl?.r_repr hreg h0 rt) ==
+     MTH.mt_get_root (mt_lift h0 mt) (Rgl?.r_repr hreg h0 rt) ==
      (mt_lift h1 mt, Rgl?.r_repr hreg h1 rt))))
 #reset-options "--z3rlimit 150 --max_fuel 1"
 let mt_get_root mt rt =
@@ -1861,9 +1916,9 @@ let mt_get_root mt rt =
       (B.loc_all_regions_from false (Rgl?.region_of hreg rt)) hh0 hh1;
     mt_preserved mt
       (B.loc_all_regions_from false (Rgl?.region_of hreg rt)) hh0 hh1;
-    High.mt_get_root_rhs_ok_true
+    MTH.mt_get_root_rhs_ok_true
       (mt_lift hh0 mt) (Rgl?.r_repr hreg hh0 rt);
-    assert (High.mt_get_root (mt_lift hh0 mt) (Rgl?.r_repr hreg hh0 rt) ==
+    assert (MTH.mt_get_root (mt_lift hh0 mt) (Rgl?.r_repr hreg hh0 rt) ==
            (mt_lift hh1 mt, Rgl?.r_repr hreg hh1 rt))
   end
   else begin
@@ -1892,7 +1947,7 @@ let mt_get_root mt rt =
 
     // correctness
     mt_safe_elts_spec hh0 0ul hs i j;
-    assert (High.construct_rhs 0
+    assert (MTH.construct_rhs 0
              (Rgl?.r_repr hvvreg hh0 hs)
              (Rgl?.r_repr hvreg hh0 rhs)
              (U32.v i) (U32.v j)
@@ -1938,15 +1993,15 @@ let mt_get_root mt rt =
     assert (mt_safe hh3 mt);
 
     // correctness
-    High.mt_get_root_rhs_ok_false
+    MTH.mt_get_root_rhs_ok_false
       (mt_lift hh0 mt) (Rgl?.r_repr hreg hh0 rt);
-    assert (High.mt_get_root (mt_lift hh0 mt) (Rgl?.r_repr hreg hh0 rt) ==
-           (High.MT (U32.v i) (U32.v j)
+    assert (MTH.mt_get_root (mt_lift hh0 mt) (Rgl?.r_repr hreg hh0 rt) ==
+           (MTH.MT (U32.v i) (U32.v j)
                     (RV.as_seq hh0 hs) true
                     (RV.as_seq hh1 rhs)
                     (Rgl?.r_repr hreg hh1 rt),
            Rgl?.r_repr hreg hh1 rt));
-    assert (High.mt_get_root (mt_lift hh0 mt) (Rgl?.r_repr hreg hh0 rt) ==
+    assert (MTH.mt_get_root (mt_lift hh0 mt) (Rgl?.r_repr hreg hh0 rt) ==
            (mt_lift hh3 mt, Rgl?.r_repr hreg hh3 rt))
   end
 
@@ -1966,7 +2021,7 @@ inline_for_extraction val path_insert:
       // correctness
       V.size_of (B.get h1 p 0) = V.size_of (B.get h0 p 0) + 1ul /\
       S.equal (lift_path h1 mtr p)
-              (High.path_insert (lift_path h0 mtr p) (Rgl?.r_repr hreg h0 hp))))
+              (MTH.path_insert (lift_path h0 mtr p) (Rgl?.r_repr hreg h0 hp))))
 let path_insert mtr p hp =
   let pv = B.index p 0ul in
   let hh0 = HST.get () in
@@ -2007,7 +2062,7 @@ val mt_path_length_step:
   k:index_t ->
   j:index_t{k <= j} ->
   actd:bool ->
-  Tot (sl:uint32_t{U32.v sl = High.mt_path_length_step (U32.v k) (U32.v j) actd})
+  Tot (sl:uint32_t{U32.v sl = MTH.mt_path_length_step (U32.v k) (U32.v j) actd})
 let mt_path_length_step k j actd =
   if j = 0ul then 0ul
   else (if k % 2ul = 0ul
@@ -2021,7 +2076,7 @@ val mt_path_length:
   j:index_t{k <= j && U32.v j < pow2 (32 - U32.v lv)} ->
   actd:bool ->
   Tot (l:uint32_t{
-        U32.v l = High.mt_path_length (U32.v k) (U32.v j) actd &&
+        U32.v l = MTH.mt_path_length (U32.v k) (U32.v j) actd &&
         l <= 32ul - lv})
       (decreases (U32.v j))
 let rec mt_path_length lv k j actd =
@@ -2058,7 +2113,7 @@ val mt_get_path_step:
      // correctness
      (mt_safe_elts_spec h0 lv hs i j;
      S.equal (lift_path h1 mtr p)
-             (High.mt_get_path_step
+             (MTH.mt_get_path_step
                (U32.v lv) (RV.as_seq h0 hs) (RV.as_seq h0 rhs)
                (U32.v i) (U32.v j) (U32.v k) (lift_path h0 mtr p) actd))))
 let mt_get_path_step lv mtr hs rhs i j k p actd =
@@ -2110,10 +2165,10 @@ val mt_get_path_:
      // correctness
      (mt_safe_elts_spec h0 lv hs i j;
      S.equal (lift_path h1 mtr p)
-             (High.mt_get_path_ (U32.v lv) (RV.as_seq h0 hs) (RV.as_seq h0 rhs)
+             (MTH.mt_get_path_ (U32.v lv) (RV.as_seq h0 hs) (RV.as_seq h0 rhs)
                (U32.v i) (U32.v j) (U32.v k) (lift_path h0 mtr p) actd))))
    (decreases (32 - U32.v lv))
-#reset-options "--z3rlimit 300 --max_fuel 1 --initial_fuel 1 --max_ifuel 2 --initial_ifuel 2"
+#reset-options "--z3rlimit 300 --max_ifuel 2 --initial_ifuel 2"
 let rec mt_get_path_ lv mtr hs rhs i j k p actd =
   let hh0 = HST.get () in
   mt_safe_elts_spec hh0 lv hs i j;
@@ -2126,7 +2181,7 @@ let rec mt_get_path_ lv mtr hs rhs i j k p actd =
     let hh1 = HST.get () in
     mt_safe_elts_spec hh0 lv hs i j;
     assert (S.equal (lift_path hh1 mtr p)
-                    (High.mt_get_path_step
+                    (MTH.mt_get_path_step
                       (U32.v lv) (RV.as_seq hh0 hs) (RV.as_seq hh0 rhs)
                       (U32.v i) (U32.v j) (U32.v k)
                       (lift_path hh0 mtr p) actd));
@@ -2146,13 +2201,13 @@ let rec mt_get_path_ lv mtr hs rhs i j k p actd =
 
     let hh2 = HST.get () in
     assert (S.equal (lift_path hh2 mtr p)
-                    (High.mt_get_path_ (U32.v lv + 1)
+                    (MTH.mt_get_path_ (U32.v lv + 1)
                       (RV.as_seq hh1 hs) (RV.as_seq hh1 rhs)
                       (U32.v i / 2) (U32.v j / 2) (U32.v k / 2)
                       (lift_path hh1 mtr p)
                       (if U32.v j % 2 = 0 then actd else true)));
     assert (S.equal (lift_path hh2 mtr p)
-                    (High.mt_get_path_ (U32.v lv)
+                    (MTH.mt_get_path_ (U32.v lv)
                       (RV.as_seq hh0 hs) (RV.as_seq hh0 rhs)
                       (U32.v i) (U32.v j) (U32.v k)
                       (lift_path hh0 mtr p) actd)))
@@ -2222,7 +2277,7 @@ val mt_get_path:
      1ul + mt_path_length 0ul idx (MT?.j (B.get h0 mt 0)) false /\
      // correctness
      (let sj, sp, srt =
-       High.mt_get_path
+       MTH.mt_get_path
          (mt_lift h0 mt) (U32.v idx) (Rgl?.r_repr hreg h0 root) in
      sj == U32.v (MT?.j (B.get h1 mt 0)) /\
      S.equal sp (lift_path h1 (B.frameOf mt) p) /\
@@ -2240,7 +2295,7 @@ let mt_get_path mt idx p root =
     (B.loc_union (mt_loc ncmt)
       (B.loc_all_regions_from false (B.frameOf root)))
     hh0 hh1;
-  assert (High.mt_get_root (mt_lift hh0 ncmt) (Rgl?.r_repr hreg hh0 root) ==
+  assert (MTH.mt_get_root (mt_lift hh0 ncmt) (Rgl?.r_repr hreg hh0 root) ==
          (mt_lift hh1 ncmt, Rgl?.r_repr hreg hh1 root));
   assert (S.equal (lift_path hh1 mtframe p) S.empty);
 
@@ -2265,7 +2320,7 @@ let mt_get_path mt idx p root =
 
   let hh2 = HST.get () in
   assert (S.equal (lift_path hh2 mtframe p)
-                  (High.path_insert
+                  (MTH.path_insert
                     (lift_path hh1 mtframe p)
                     (S.index (S.index (RV.as_seq hh1 hs) 0) (U32.v idx - U32.v ofs))));
   Rgl?.r_sep hreg root (path_loc p) hh1 hh2;
@@ -2289,7 +2344,7 @@ let mt_get_path mt idx p root =
          1ul + mt_path_length 0ul idx (MT?.j (B.get hh0 ncmt 0)) false);
   assert (S.length (lift_path hh3 mtframe p) ==
          S.length (lift_path hh2 mtframe p) +
-         High.mt_path_length (U32.v idx) (U32.v (MT?.j (B.get hh0 ncmt 0))) false);
+         MTH.mt_path_length (U32.v idx) (U32.v (MT?.j (B.get hh0 ncmt 0))) false);
 
   assert (modifies (loc_union
                      (loc_union
@@ -2306,10 +2361,10 @@ let mt_get_path mt idx p root =
   // correctness
   mt_safe_elts_spec hh2 0ul hs i j;
   assert (S.equal (lift_path hh3 mtframe p)
-                  (High.mt_get_path_ 0 (RV.as_seq hh2 hs) (RV.as_seq hh2 rhs)
+                  (MTH.mt_get_path_ 0 (RV.as_seq hh2 hs) (RV.as_seq hh2 rhs)
                     (U32.v i) (U32.v j) (U32.v idx)
                     (lift_path hh2 mtframe p) false));
-  assert (High.mt_get_path
+  assert (MTH.mt_get_path
            (mt_lift hh0 ncmt) (U32.v idx) (Rgl?.r_repr hreg hh0 root) ==
          (U32.v (MT?.j (B.get hh3 ncmt 0)),
          lift_path hh3 mtframe p,
@@ -2372,7 +2427,7 @@ val mt_flush_to_:
      // correctness
      (mt_safe_elts_spec h0 lv hs pi (Ghost.reveal j);
      S.equal (RV.as_seq h1 hs)
-             (High.mt_flush_to_
+             (MTH.mt_flush_to_
                (U32.v lv) (RV.as_seq h0 hs) (U32.v pi)
                (U32.v i) (U32.v (Ghost.reveal j))))))
    (decreases (U32.v i))
@@ -2542,14 +2597,14 @@ let rec mt_flush_to_ lv hs pi i j =
     // 3-1) Correctness
     mt_safe_elts_spec hh2 (lv + 1ul) hs (pi / 2ul) (Ghost.reveal j / 2ul);
     assert (S.equal (RV.as_seq hh3 hs)
-                    (High.mt_flush_to_ (U32.v lv + 1) (RV.as_seq hh2 hs)
+                    (MTH.mt_flush_to_ (U32.v lv + 1) (RV.as_seq hh2 hs)
                       (U32.v pi / 2) (U32.v i / 2) (U32.v (Ghost.reveal j) / 2)));
     mt_safe_elts_spec hh0 lv hs pi (Ghost.reveal j);
-    High.mt_flush_to_rec
+    MTH.mt_flush_to_rec
       (U32.v lv) (RV.as_seq hh0 hs)
       (U32.v pi) (U32.v i) (U32.v (Ghost.reveal j));
     assert (S.equal (RV.as_seq hh3 hs)
-                    (High.mt_flush_to_ (U32.v lv) (RV.as_seq hh0 hs)
+                    (MTH.mt_flush_to_ (U32.v lv) (RV.as_seq hh0 hs)
                       (U32.v pi) (U32.v i) (U32.v (Ghost.reveal j))))
   end
 #reset-options
@@ -2582,7 +2637,7 @@ let mt_flush_to_pre mt idx =
   let mtv = !*mt in
   mt_flush_to_pre_nst mtv idx
 
-#reset-options "--z3rlimit 20 --initial_fuel 1 --max_fuel 1 --initial_ifuel 0 --max_ifuel 0"
+#push-options "--z3rlimit 20 --initial_ifuel 0 --max_ifuel 0"
 val mt_flush_to:
   mt:mt_p ->
   idx:offset_t ->
@@ -2596,9 +2651,10 @@ val mt_flush_to:
      (let mtv = B.get h0 mt 0 in
       let off = MT?.offset mtv in
       let idx = split_offset off idx in
-      High.mt_flush_to (mt_lift h0 mt) (U32.v idx) == mt_lift h1 mt)))
+      MTH.mt_flush_to (mt_lift h0 mt) (U32.v idx) == mt_lift h1 mt)))
+#pop-options
 
-#reset-options "--z3rlimit 100 --initial_fuel 1 --max_fuel 1 --initial_ifuel 0 --max_ifuel 0"
+#push-options "--z3rlimit 100 --initial_ifuel 0 --max_ifuel 0"
 let mt_flush_to mt idx =
   let hh0 = HST.get () in
   let mtv = !*mt in
@@ -2635,6 +2691,7 @@ let mt_flush_to mt idx =
   RV.as_seq_preserved (MT?.rhs mtv) (B.loc_buffer mt) hh1 hh2;
   Rgl?.r_sep hreg (MT?.mroot mtv) (B.loc_buffer mt) hh1 hh2;
   mt_safe_elts_preserved 0ul hs idx (MT?.j mtv) (B.loc_buffer mt) hh1 hh2
+#pop-options
 
 private inline_for_extraction
 val mt_flush_pre_nst: mt:merkle_tree -> Tot bool
@@ -2643,7 +2700,7 @@ let mt_flush_pre_nst mt = MT?.j mt > MT?.i mt
 val mt_flush_pre: mt:const_mt_p -> HST.ST bool (requires (fun h0 -> mt_safe h0 (CB.cast mt))) (ensures (fun _ _ _ -> True))
 let mt_flush_pre mt = mt_flush_pre_nst !*(CB.cast mt)
 
-#reset-options "--z3rlimit 200 --initial_fuel 1 --max_fuel 1 --initial_ifuel 0 --max_ifuel 0"
+#push-options "--z3rlimit 200 --initial_ifuel 0 --max_ifuel 0"
 val mt_flush:
   mt:mt_p ->
   HST.ST unit
@@ -2653,7 +2710,7 @@ val mt_flush:
      modifies (mt_loc mt) h0 h1 /\
      mt_safe h1 mt /\
      // correctness
-     High.mt_flush (mt_lift h0 mt) == mt_lift h1 mt))
+     MTH.mt_flush (mt_lift h0 mt) == mt_lift h1 mt))
 let mt_flush mt =
   let mtv = !*mt in
   let off = MT?.offset mtv in
@@ -2664,12 +2721,12 @@ let mt_flush mt =
   assert (UInt.fits (U64.v off + U32.v j1) 64);
   let jo = join_offset off j1 in
   mt_flush_to mt jo
-#reset-options
+#pop-options
 
 
 /// Retraction
 
-#reset-options "--z3rlimit 50 --initial_fuel 1 --max_fuel 1 --initial_ifuel 0 --max_ifuel 0"
+#push-options "--z3rlimit 50 --initial_ifuel 0 --max_ifuel 0"
 private
 val mt_retract_to_:
   hs:hash_vv{V.size_of hs = merkle_tree_size_lg} ->
@@ -2692,12 +2749,13 @@ val mt_retract_to_:
      // correctness
      (mt_safe_elts_spec h0 lv hs i j;
      S.equal (RV.as_seq h1 hs)
-             (High.mt_retract_to_
+             (MTH.mt_retract_to_
                (RV.as_seq h0 hs) (U32.v lv)
                (U32.v i) (U32.v s) (U32.v j)))
      ))
    (decreases (U32.v merkle_tree_size_lg - U32.v lv))
-#reset-options "--z3rlimit 250  --initial_fuel 1 --max_fuel 1 --initial_ifuel 1 --max_ifuel 1"
+#pop-options
+#push-options "--z3rlimit 250 --initial_ifuel 1 --max_ifuel 1"
 private
 let rec mt_retract_to_ hs lv i s j =
   let hh0 = HST.get () in
@@ -2858,13 +2916,13 @@ let rec mt_retract_to_ hs lv i s j =
       mt_safe_elts_spec hh2 (lv + 1ul) hs (i / 2ul) (j / 2ul);
       assert (U32.v lv + 1 < S.length (RV.as_seq hh3 hs) ==>
                     S.equal (RV.as_seq hh3 hs)
-                      (High.mt_retract_to_ (RV.as_seq hh2 hs) (U32.v lv + 1)
+                      (MTH.mt_retract_to_ (RV.as_seq hh2 hs) (U32.v lv + 1)
                         (U32.v i / 2) (U32.v s / 2) (U32.v j / 2)));
       assert (RV.rv_inv hh0 hs);
       assert (mt_safe_elts hh0 lv hs i j);
       mt_safe_elts_spec hh0 lv hs i j;
       assert (S.equal (RV.as_seq hh3 hs)
-                      (High.mt_retract_to_ (RV.as_seq hh0 hs) (U32.v lv)
+                      (MTH.mt_retract_to_ (RV.as_seq hh0 hs) (U32.v lv)
                         (U32.v i) (U32.v s) (U32.v j)))
     end
     else begin
@@ -2876,12 +2934,12 @@ let rec mt_retract_to_ hs lv i s j =
       assert (RV.rv_inv hh3 hs /\ mt_safe_elts hh3 lv hs i s);
       mt_safe_elts_spec hh0 lv hs i j;
       assert (S.equal (RV.as_seq hh3 hs)
-                      (High.mt_retract_to_
+                      (MTH.mt_retract_to_
                       (RV.as_seq hh0 hs) (U32.v lv)
                       (U32.v i) (U32.v s) (U32.v j)))
     end
   end
-#reset-options
+#pop-options
 
 private inline_for_extraction
 val mt_retract_to_pre_nst: mtv:merkle_tree -> r:offset_t -> Tot bool
@@ -2899,7 +2957,7 @@ let mt_retract_to_pre mt r =
   let mtv = !*mt in
   mt_retract_to_pre_nst mtv r
 
-#reset-options "--z3rlimit 20 --initial_fuel 1 --max_fuel 1 --initial_ifuel 0 --max_ifuel 0"
+#push-options "--z3rlimit 100 --initial_ifuel 0 --max_ifuel 0"
 val mt_retract_to:
   mt:mt_p ->
   r:offset_t ->
@@ -2913,8 +2971,7 @@ val mt_retract_to:
      (let mtv = B.get h0 mt 0 in
       let off = MT?.offset mtv in
       let r = split_offset off r in
-      High.mt_retract_to (mt_lift h0 mt) (U32.v r) == mt_lift h1 mt)))
-#reset-options "--z3rlimit 100 --initial_fuel 1 --max_fuel 1 --initial_ifuel 0 --max_ifuel 0"
+      MTH.mt_retract_to (mt_lift h0 mt) (U32.v r) == mt_lift h1 mt)))
 let mt_retract_to mt r =
   let hh0 = HST.get () in
   let mtv = !*mt in
@@ -2950,11 +3007,11 @@ let mt_retract_to mt r =
   RV.as_seq_preserved (MT?.rhs mtv) (B.loc_buffer mt) hh1 hh2;
   Rgl?.r_sep hreg (MT?.mroot mtv) (B.loc_buffer mt) hh1 hh2;
   mt_safe_elts_preserved 0ul hs (MT?.i mtv) (r+1ul) (B.loc_buffer mt) hh1 hh2
-#reset-options
+#pop-options
 
 /// Client-side verification
 
-#reset-options "--z3rlimit 50 --initial_fuel 1 --max_fuel 1 --initial_ifuel 0 --max_ifuel 0"
+#push-options "--z3rlimit 200 --initial_ifuel 0 --max_ifuel 0"
 private
 val mt_verify_:
   k:index_t ->
@@ -2982,9 +3039,8 @@ val mt_verify_:
      Rgl?.r_inv hreg h1 acc /\
      // correctness
      Rgl?.r_repr hreg h1 acc ==
-     High.mt_verify_ (U32.v k) (U32.v j) (lift_path h0 mtr p)
+     MTH.mt_verify_ (U32.v k) (U32.v j) (lift_path h0 mtr p)
        (U32.v ppos) (Rgl?.r_repr hreg h0 acc) actd))
-#reset-options "--z3rlimit 200 --max_fuel 1"
 private
 let rec mt_verify_ k j mtr p ppos acc actd hash_fun =
   let ncp:path_p = CB.cast p in
@@ -3002,7 +3058,7 @@ let rec mt_verify_ k j mtr p ppos acc actd hash_fun =
              (B.loc_all_regions_from false (B.frameOf acc)) hh0 hh1;
            lift_path_index hh0 mtr ncp ppos;
            assert (Rgl?.r_repr hreg hh1 acc ==
-                  High.hash_2 (Rgl?.r_repr hreg hh0 acc)
+                  MTH.sha256_compress (Rgl?.r_repr hreg hh0 acc)
                               (S.index (lift_path hh0 mtr ncp) (U32.v ppos)));
            mt_verify_ (k / 2ul) (j / 2ul) mtr p (ppos + 1ul) acc nactd hash_fun
          end
@@ -3015,10 +3071,11 @@ let rec mt_verify_ k j mtr p ppos acc actd hash_fun =
            (B.loc_all_regions_from false (B.frameOf acc)) hh0 hh1;
          lift_path_index hh0 mtr ncp ppos;
          assert (Rgl?.r_repr hreg hh1 acc ==
-                High.hash_2 (S.index (lift_path hh0 mtr ncp) (U32.v ppos))
+                MTH.sha256_compress (S.index (lift_path hh0 mtr ncp) (U32.v ppos))
                             (Rgl?.r_repr hreg hh0 acc));
          mt_verify_ (k / 2ul) (j / 2ul) mtr p (ppos + 1ul) acc nactd hash_fun
        end)
+#pop-options
 
 private inline_for_extraction
 val mt_verify_pre_nst: mt:merkle_tree -> k:offset_t -> j:offset_t -> p:V.vector hash -> rt:hash -> Tot bool
@@ -3060,7 +3117,7 @@ let mt_verify_pre mt k j mtr p rt =
 // Note that `mt_path_length` is given as a precondition of this operation.
 // This is a postcondition of `mt_get_path` so we can call `mt_verify` with
 // every path generated by `mt_get_path`.
-#reset-options "--z3rlimit 150 --initial_fuel 1 --max_fuel 1 --initial_ifuel 0 --max_ifuel 0"
+#push-options "--z3rlimit 200 --initial_ifuel 0 --max_ifuel 0"
 val mt_verify:
   mt:const_mt_p ->
   k:uint64_t ->
@@ -3091,9 +3148,8 @@ val mt_verify:
      (let mtv = B.get h0 mt 0 in
       let k = split_offset (MT?.offset mtv) k in
       let j = split_offset (MT?.offset mtv) j in
-      b <==> High.mt_verify (U32.v k) (U32.v j)
+      b <==> MTH.mt_verify (U32.v k) (U32.v j)
              (lift_path h0 mtr p) (Rgl?.r_repr hreg h0 rt))))
-#reset-options "--z3rlimit 200 --initial_fuel 1 --max_fuel 1 --initial_ifuel 0 --max_ifuel 0"
 let mt_verify mt k j mtr p rt =
   let ncmt = CB.cast mt in
   let ncp = CB.cast p in
@@ -3114,9 +3170,9 @@ let mt_verify mt k j mtr p rt =
   mt_verify_ k j mtr p 1ul ih false (MT?.hash_fun mtv);
   let hh2 = HST.get () in
   assert (Rgl?.r_repr hreg hh2 ih ==
-         High.mt_verify_ (U32.v k) (U32.v j) (lift_path hh1 mtr ncp)
+         MTH.mt_verify_ (U32.v k) (U32.v j) (lift_path hh1 mtr ncp)
            1 (Rgl?.r_repr hreg hh1 ih) false);
-  let r = Lib.ByteBuffer.lbytes_eq #hash_size ih rt in
+  let r = Lib.ByteBuffer.lbytes_eq #_ ih rt in
   Rgl?.r_free hreg ih;
   r
-
+#pop-options
